Tree Bags implemented, missing correctness proofs.

src/QueryStructure/Refinements/Bags/TreeBags.v
@@ -4,6 +4,7 @@ Require Import FMapInterface Coq.FSets.FMapFacts.
 
 Unset Implicit Arguments.
 
+
 Module TreeBag (Import M: WS).
   Module Import BasicFacts := WFacts_fun E M.
   Module Import BasicProperties := WProperties_fun E M.
@@ -11,206 +12,218 @@ Module TreeBag (Import M: WS).
 
   Definition TKey := key.
 
-  Context {TBag : Type}
-          {TItem : Type}
-          {TBagSearchTerm : Type}
-          {TBagUpdateTerm : Type}.
-  Variables (projection: TItem -> TKey)            
-            (bags_bag: Bag TBag TItem TBagSearchTerm TBagUpdateTerm).
+  Section TreeBagDefinitions.
 
-  Definition IndexedTreeConsistency fmap :=
-    forall (key: TKey) (bag: TBag),
-      MapsTo key bag fmap ->
-      forall (item: TItem),
+    Context {TBag : Type}
+            {TItem : Type}
+            {TBagSearchTerm : Type}
+            {TBagUpdateTerm : Type}.
+    Variable (projection: TItem -> TKey).
+
+    (* A class for Bags whose update functions preserve the key *)
+    Class KeyPreservingUpdateBag :=
+      { KeyPreserving_bag :> Bag TBag TItem TBagSearchTerm TBagUpdateTerm;
+        KeyPreserving_Proof :
+          forall K item updateTerm searchTerm,
+            E.eq (projection item) K
+            -> bfind_matcher searchTerm item = true
+            -> E.eq (projection (bupdate_transform updateTerm item)) K }.
+
+    Variables (bags_bag: KeyPreservingUpdateBag).
+
+    Definition IndexedTreeConsistency fmap :=
+      forall (key: TKey) (bag: TBag),
+        MapsTo key bag fmap ->
+        forall (item: TItem),
+          List.In item (benumerate bag) ->
+          E.eq (projection item) key.
+
+    Record IndexedBag :=
+      { ifmap        : t TBag;
+        iconsistency : IndexedTreeConsistency ifmap
+      }.
+
+    Definition KeyFilter (key: TKey) :=
+      (fun x : TItem => if E.eq_dec (projection x) key then true else false).
+
+    Lemma KeyFilter_beq :
+      forall beq,
+        (forall x y, reflect (E.eq x y) (beq x y)) ->
+        (forall key (item: TItem),
+           KeyFilter key item = beq (projection item) key).
+    Proof.
+      intros beq spec key item.
+      specialize (spec (projection item) key).
+      unfold KeyFilter.
+      destruct spec as [ is_eq | neq ];
+        destruct (F.eq_dec _ _); intuition.
+    Qed.
+
+    Lemma iconsistency_empty :
+      IndexedTreeConsistency (empty TBag).
+    Proof.
+      unfold IndexedTreeConsistency;
+      intros; rewrite empty_mapsto_iff in *; exfalso; trivial.
+    Qed.
+
+    Lemma consistency_key_eq :
+      forall (container : IndexedBag),
+      forall (key: TKey) bag item,
+        MapsTo key bag (ifmap container) ->
         List.In item (benumerate bag) ->
         E.eq (projection item) key.
+    Proof.
+      intros.
+      destruct container as [? consistent].
+      unfold IndexedTreeConsistency in consistent.
+      eapply consistent; eauto.
+    Qed.
 
-  Record IndexedBag :=
-    { ifmap        : t TBag;
-      iconsistency : IndexedTreeConsistency ifmap
-    }.
+    Ltac destruct_if :=
+      match goal with
+          [ |- context [ if ?cond then _ else _ ] ] => destruct cond
+      end.
 
-  Definition KeyFilter (key: TKey) :=
-    (fun x : TItem => if E.eq_dec (projection x) key then true else false).
+    Lemma KeyFilter_true :
+      forall k item,
+        KeyFilter k item = true <-> E.eq (projection item) k.
+    Proof.
+      unfold KeyFilter; intros;
+      destruct_if; intros; intuition.
+    Qed.
 
-  Lemma KeyFilter_beq :
-    forall beq,
-      (forall x y, reflect (E.eq x y) (beq x y)) ->
-      (forall key (item: TItem),
-         KeyFilter key item = beq (projection item) key).
-  Proof.
-    intros beq spec key item.
-    specialize (spec (projection item) key).
-    unfold KeyFilter.
-    destruct spec as [ is_eq | neq ];
-      destruct (F.eq_dec _ _); intuition.
-  Qed.
+    Lemma KeyFilter_false :
+      forall k item,
+        KeyFilter k item = false <-> ~ E.eq (projection item) k.
+    Proof.
+      unfold KeyFilter; intros;
+      destruct_if; intros; intuition.
+    Qed.
 
-  Lemma iconsistency_empty :
-      IndexedTreeConsistency (empty TBag).
-  Proof.
-    unfold IndexedTreeConsistency;
-    intros; rewrite empty_mapsto_iff in *; exfalso; trivial.
-  Qed.
+    Definition IndexedBag_bempty :=
+      {| ifmap        := empty TBag;
+         iconsistency := iconsistency_empty |}.
 
-  Lemma consistency_key_eq :
-    forall (container : IndexedBag),
-    forall (key: TKey) bag item,
-      MapsTo key bag (ifmap container) ->
-      List.In item (benumerate bag) ->
-      E.eq (projection item) key.
-  Proof.
-    intros.
-    destruct container as [? consistent].
-    unfold IndexedTreeConsistency in consistent.
-    eapply consistent; eauto.
-  Qed.
+    Definition IndexedBag_bstar :=
+      (@None TKey, bstar (Bag := KeyPreserving_bag)).
 
-  Ltac destruct_if :=
-    match goal with
-        [ |- context [ if ?cond then _ else _ ] ] => destruct cond
-    end.
+    Definition IndexedBag_bid :=
+      (@None TKey, bid (Bag := KeyPreserving_bag)).
 
-  Lemma KeyFilter_true :
-    forall k item,
-      KeyFilter k item = true <-> E.eq (projection item) k.
-  Proof.
-    unfold KeyFilter; intros;
-    destruct_if; intros; intuition.
-  Qed.
+    Definition IndexedBag_bfind_matcher
+               (key_searchterm: (option TKey) * TBagSearchTerm) (item: TItem) :=
+      let (key_option, search_term) := key_searchterm in
+      match key_option with
+        | Some k => KeyFilter k item
+        | None   => true
+      end && (bfind_matcher search_term item).
 
-  Lemma KeyFilter_false :
-    forall k item,
-      KeyFilter k item = false <-> ~ E.eq (projection item) k.
-  Proof.
-    unfold KeyFilter; intros;
-    destruct_if; intros; intuition.
-  Qed.
+    Definition IndexedBag_benumerate
+               (container: IndexedBag) :=
+      flatten (List.map benumerate (Values (ifmap container))).
 
-  Definition IndexedBag_bempty :=
-    {| ifmap        := empty TBag;
-       iconsistency := iconsistency_empty |}.
+    Definition IndexedBag_bfind
+               (container: IndexedBag)
+               (key_searchterm: (option TKey) * TBagSearchTerm) :=
+      let (key_option, search_term) := key_searchterm in
+      match key_option with
+        | Some k =>
+          match find k (ifmap container) with
+            | Some bag => bfind (Bag := KeyPreserving_bag) bag search_term
+            | None     => nil
+          end
+        | None   =>
+          flatten (List.map (fun bag => bfind (Bag := KeyPreserving_bag) bag search_term) (Values (ifmap container)))
+      end.
 
-  Definition IndexedBag_bstar :=
-    (@None TKey, @bstar _ _ _ _ bags_bag).
+    Lemma InA_mapsto_add {Value} :
+      forall bag' kv k' (v' : Value),
+        InA (@eq_key_elt _) kv (elements (add k' v' bag')) ->
+        eq_key_elt kv (k', v') \/
+        (~ E.eq (fst kv) k' /\
+         InA (@eq_key_elt _) kv (elements bag')).
+    Proof.
+      intros.
+      destruct kv as [k v]; apply elements_2 in H.
+      apply add_mapsto_iff in H; intuition; subst;
+      [left; split; simpl; eauto |
+       right; eauto using elements_1].
+    Qed.
 
-  Definition IndexedBag_bid :=
-    (@None TKey, @bid _ _ _ _ bags_bag).
-
-  Definition IndexedBag_bfind_matcher
-             (key_searchterm: (option TKey) * TBagSearchTerm) (item: TItem) :=
-    let (key_option, search_term) := key_searchterm in
-    match key_option with
-      | Some k => KeyFilter k item
-      | None   => true
-    end && (bfind_matcher search_term item).
-
-  Definition IndexedBag_benumerate
-             (container: IndexedBag) :=
-    flatten (List.map benumerate (Values (ifmap container))).
-
-  Definition IndexedBag_bfind
-             (container: IndexedBag)
-             (key_searchterm: (option TKey) * TBagSearchTerm) :=
-    let (key_option, search_term) := key_searchterm in
-    match key_option with
-      | Some k =>
-        match find k (ifmap container) with
-          | Some bag => @bfind _ _ _ _ bags_bag bag search_term
-          | None     => nil
-        end
-      | None   =>
-        flatten (List.map (fun bag =>  @bfind _ _ _ _ bags_bag bag search_term) (Values (ifmap container)))
-    end.
-
-  Lemma InA_mapsto_add {Value} : 
-    forall bag' kv k' (v' : Value),
-      InA (@eq_key_elt _) kv (elements (add k' v' bag')) -> 
-      eq_key_elt kv (k', v') \/
-      (~ E.eq (fst kv) k' /\
-       InA (@eq_key_elt _) kv (elements bag')).
-  Proof.
-    intros.
-    destruct kv as [k v]; apply elements_2 in H.
-    apply add_mapsto_iff in H; intuition; subst;
-    [left; split; simpl; eauto | 
-     right; eauto using elements_1].
-  Qed.
-
-  Lemma InA_mapsto_add' {Value} : 
-    forall bag' kv k' (v' : Value),
-      (eq_key_elt kv (k', v') \/
-       (~ E.eq (fst kv) k' /\
-        InA (@eq_key_elt _) kv (elements bag'))) 
-      -> InA (@eq_key_elt _) kv (elements (add k' v' bag')).
-  Proof.
-    intros; destruct kv as [k v]; apply elements_1; 
-    apply add_mapsto_iff; intuition;
-    [destruct H0; eauto 
-    | right; intuition; apply elements_2; eauto].
-  Qed.
+    Lemma InA_mapsto_add' {Value} :
+      forall bag' kv k' (v' : Value),
+        (eq_key_elt kv (k', v') \/
+         (~ E.eq (fst kv) k' /\
+          InA (@eq_key_elt _) kv (elements bag')))
+        -> InA (@eq_key_elt _) kv (elements (add k' v' bag')).
+    Proof.
+      intros; destruct kv as [k v]; apply elements_1;
+      apply add_mapsto_iff; intuition;
+      [destruct H0; eauto
+      | right; intuition; apply elements_2; eauto].
+    Qed.
 
     Lemma InA_app_swap {A} eqA :
-      Equivalence eqA 
-      -> forall (a : A) l l', 
+      Equivalence eqA
+      -> forall (a : A) l l',
            InA eqA a (l ++ l') -> InA eqA a (l' ++ l).
     Proof.
-      intros; eapply InA_app_iff; 
+      intros; eapply InA_app_iff;
       eapply InA_app_iff in H0; eauto; intuition.
     Qed.
-    
+
     Lemma InA_app_cons_swap {A} eqA :
-      Equivalence eqA 
-      -> forall (a a' : A) l l', 
+      Equivalence eqA
+      -> forall (a a' : A) l l',
            InA eqA a (l ++ (a' :: l')) <-> InA eqA a ((a' :: l) ++ l').
     Proof.
       split; intros.
       - eapply InA_app_swap; eauto.
-        intros; eapply InA_app_iff; 
+        intros; eapply InA_app_iff;
         eapply InA_app_iff in H0; eauto; intuition.
         inversion H; subst; eauto.
       - eapply InA_app_swap; eauto.
-        intros; eapply InA_app_iff; 
+        intros; eapply InA_app_iff;
         eapply InA_app_iff in H0; eauto; intuition.
         inversion H; subst; eauto.
     Qed.
 
-  Lemma Permutation_InA_cons {Value} : 
-    forall l (l' : list (key * Value)), 
-      NoDupA (@eq_key _) l
-      -> NoDupA (@eq_key _) l'
-      -> (forall k v, 
-            InA (@eq_key_elt _) (k, v) l' <-> 
-            (InA (@eq_key_elt _) (k, v) l))
-      -> Permutation (List.map snd l') 
-                     (List.map snd l).
-  Proof.
-    induction l; intros.
-    destruct l'.
-    constructor.
-    assert (InA (eq_key_elt (elt:=Value)) (fst p, snd p) []) as H2
-      by (eapply H1; left; split; reflexivity); inversion H2.
-    destruct a as [k v].
-    assert (InA (eq_key_elt (elt:=Value)) (k, v) l') as H2
-      by (eapply H1; econstructor; split; reflexivity).
-    destruct (InA_split H2) as [l'1 [kv [l'2 [eq_kv eq_l]]]]; subst.
-    rewrite <- Permutation_middle; simpl.
-    destruct eq_kv; simpl in *; subst; constructor.
-    eapply NoDupA_swap in H0; eauto using eqk_equiv.
-    inversion H0; inversion H; subst; apply IHl; eauto.
-    assert (forall (k0 : key) (v : Value),
-              InA (eq_key_elt (elt:=Value)) (k0, v) (kv :: (l'1 ++ l'2)) <->
-              InA (eq_key_elt (elt:=Value)) (k0, v) ((k, snd kv) :: l)) by 
-        (split; intros;
-         [ eapply H1; eapply InA_app_cons_swap
-         | eapply H1 in H4; eapply InA_app_cons_swap in H4 ]; eauto using eqke_equiv).
-    split; intros. 
-    + generalize (proj1 (H4 k0 v) (InA_cons_tl _ H5)); intros.
-      inversion H8; subst; eauto.
-      destruct H12; simpl in *.
-      elimtype False; apply H6.
-      revert H5 H9 H3; clear; induction (l'1 ++ l'2); intros;
-      inversion H5; subst;
+    Lemma Permutation_InA_cons {Value} :
+      forall l (l' : list (key * Value)),
+        NoDupA (@eq_key _) l
+        -> NoDupA (@eq_key _) l'
+        -> (forall k v,
+              InA (@eq_key_elt _) (k, v) l' <->
+              (InA (@eq_key_elt _) (k, v) l))
+        -> Permutation (List.map snd l')
+                       (List.map snd l).
+    Proof.
+      induction l; intros.
+      destruct l'.
+      constructor.
+      assert (InA (eq_key_elt (elt:=Value)) (fst p, snd p) []) as H2
+                                                                 by (eapply H1; left; split; reflexivity); inversion H2.
+      destruct a as [k v].
+      assert (InA (eq_key_elt (elt:=Value)) (k, v) l') as H2
+                                                         by (eapply H1; econstructor; split; reflexivity).
+      destruct (InA_split H2) as [l'1 [kv [l'2 [eq_kv eq_l]]]]; subst.
+      rewrite <- Permutation_middle; simpl.
+      destruct eq_kv; simpl in *; subst; constructor.
+      eapply NoDupA_swap in H0; eauto using eqk_equiv.
+      inversion H0; inversion H; subst; apply IHl; eauto.
+      assert (forall (k0 : key) (v : Value),
+                InA (eq_key_elt (elt:=Value)) (k0, v) (kv :: (l'1 ++ l'2)) <->
+                InA (eq_key_elt (elt:=Value)) (k0, v) ((k, snd kv) :: l)) by
+          (split; intros;
+           [ eapply H1; eapply InA_app_cons_swap
+           | eapply H1 in H4; eapply InA_app_cons_swap in H4 ]; eauto using eqke_equiv).
+      split; intros.
+      + generalize (proj1 (H4 k0 v) (InA_cons_tl _ H5)); intros.
+        inversion H8; subst; eauto.
+        destruct H12; simpl in *.
+        elimtype False; apply H6.
+        revert H5 H9 H3; clear; induction (l'1 ++ l'2); intros;
+        inversion H5; subst;
         [ constructor; destruct H0; simpl in *; unfold eq_key;
           rewrite <- H3, <- H9; eauto
         | constructor 2; eauto ].
@@ -219,557 +232,572 @@ Module TreeBag (Import M: WS).
         inversion H8; subst; eauto.
         destruct H12; simpl in *.
         elimtype False; apply H10.
-        revert H5 H9 H3; clear; induction l; intros; 
+        revert H5 H9 H3; clear; induction l; intros;
         inversion H5; subst;
         [ constructor; destruct H0; simpl in *; unfold eq_key;
           simpl; rewrite <- H, H9; eauto
         | constructor 2; eauto ].
-  Qed.
+    Qed.
 
-  Lemma FMap_Insert_fold_add {Value}
-  : forall (f : Value -> Value) (bag : t Value) bag', 
-      (forall (k : key), InA E.eq k (List.map fst (elements bag))
-                  -> ~ In k bag')
-      -> Permutation 
-           (List.map snd (elements (fold (fun k bag'' r' => add k (f bag'') r') 
-                           bag bag')))
-           (List.map snd ((List.map (fun kv => (fst kv, f (snd kv))) (elements bag)) ++ elements bag')).
-  Proof.
-    intros.
-    intros; rewrite fold_1.
-    generalize (elements_3w bag) as NoDupl.
-    revert bag' H; induction (elements bag); simpl; intros.
-    reflexivity.
-    rewrite IHl, Permutation_cons_app; 
-      try (rewrite List.map_app; reflexivity).
-    rewrite List.map_app, List.map_map.
-    apply Permutation_app; try reflexivity.
-    apply (Permutation_InA_cons ((fst a, f (snd a)) :: elements bag'));
-      eauto using elements_3w.
-    econstructor; eauto using elements_3w.
-    unfold not; intros; eapply (H (fst a)); 
-    [ constructor; reflexivity 
-    | eapply elements_in_iff; revert H0; clear; intro; induction H0].
-    repeat econstructor; eauto.
-    destruct IHInA; econstructor; econstructor 2; eauto.
-    split; intros.
-    apply InA_mapsto_add in H0; intuition.
-    inversion H0; subst; eapply InA_mapsto_add'; intuition.
-    right; intuition.
-    eapply H; simpl.
-    econstructor; reflexivity.
-    eapply elements_in_iff; revert H2 H1; clear; intros;
-    induction H2.
-    destruct H; repeat econstructor; eauto.
-    destruct IHInA; econstructor; econstructor 2; eauto.
-    unfold not; intros.
-    apply add_in_iff in H1; destruct H1.
-    inversion NoDupl; subst; rewrite <- H1 in H0; eapply H4.
-    revert H0; clear; induction l; intros; inversion H0; subst.
-    constructor; eauto.
-    econstructor 2; eauto.
-    eapply H; eauto.
-    inversion NoDupl; eauto.
-  Qed.
+    Lemma FMap_Insert_fold_add {Value}
+    : forall (f : Value -> Value) (bag : t Value) bag',
+        (forall (k : key), InA E.eq k (List.map fst (elements bag))
+                           -> ~ In k bag')
+        -> Permutation
+             (List.map snd (elements (fold (fun k bag'' r' => add k (f bag'') r')
+                                           bag bag')))
+             (List.map snd ((List.map (fun kv => (fst kv, f (snd kv))) (elements bag)) ++ elements bag')).
+    Proof.
+      intros.
+      intros; rewrite fold_1.
+      generalize (elements_3w bag) as NoDupl.
+      revert bag' H; induction (elements bag); simpl; intros.
+      reflexivity.
+      rewrite IHl, Permutation_cons_app;
+        try (rewrite List.map_app; reflexivity).
+      rewrite List.map_app, List.map_map.
+      apply Permutation_app; try reflexivity.
+      apply (Permutation_InA_cons ((fst a, f (snd a)) :: elements bag'));
+        eauto using elements_3w.
+      econstructor; eauto using elements_3w.
+      unfold not; intros; eapply (H (fst a));
+      [ constructor; reflexivity
+      | eapply elements_in_iff; revert H0; clear; intro; induction H0].
+      repeat econstructor; eauto.
+      destruct IHInA; econstructor; econstructor 2; eauto.
+      split; intros.
+      apply InA_mapsto_add in H0; intuition.
+      inversion H0; subst; eapply InA_mapsto_add'; intuition.
+      right; intuition.
+      eapply H; simpl.
+      econstructor; reflexivity.
+      eapply elements_in_iff; revert H2 H1; clear; intros;
+      induction H2.
+      destruct H; repeat econstructor; eauto.
+      destruct IHInA; econstructor; econstructor 2; eauto.
+      unfold not; intros.
+      apply add_in_iff in H1; destruct H1.
+      inversion NoDupl; subst; rewrite <- H1 in H0; eapply H4.
+      revert H0; clear; induction l; intros; inversion H0; subst.
+      constructor; eauto.
+      econstructor 2; eauto.
+      eapply H; eauto.
+      inversion NoDupl; eauto.
+    Qed.
 
-  Lemma FMap_fold_add_MapsTo_NIn {Value}
-  : forall (f : Value -> Value) l k v bag', 
-      ~ InA (@eq_key _) (k,v) (List.map (fun kv => (fst kv, f (snd kv))) l)
-      -> (MapsTo k v (fold_left (fun a p => add (fst p) (f (snd p)) a) l bag')
-                      <-> MapsTo k v bag').
-  Proof.
-    unfold eq_key; intros; revert k v bag' H.
-    induction l; simpl; intros; split; eauto.
-    intros; assert (MapsTo k v (add (fst a) (f (snd a)) bag')).
-    apply IHl; 
-      [unfold not; intros; apply H; constructor 2; eauto
-      | eauto].
-    apply add_mapsto_iff in H1; intuition; subst.
-    intros; eapply IHl; eauto using add_2.
-  Qed.    
+    Lemma FMap_fold_add_MapsTo_NIn {Value}
+    : forall (f : Value -> Value) l k v bag',
+        ~ InA (@eq_key _) (k,v) (List.map (fun kv => (fst kv, f (snd kv))) l)
+        -> (MapsTo k v (fold_left (fun a p => add (fst p) (f (snd p)) a) l bag')
+            <-> MapsTo k v bag').
+    Proof.
+      unfold eq_key; intros; revert k v bag' H.
+      induction l; simpl; intros; split; eauto.
+      intros; assert (MapsTo k v (add (fst a) (f (snd a)) bag')).
+      apply IHl;
+        [unfold not; intros; apply H; constructor 2; eauto
+        | eauto].
+      apply add_mapsto_iff in H1; intuition; subst.
+      intros; eapply IHl; eauto using add_2.
+    Qed.
 
-  Lemma FMap_fold_add_MapsTo_In {Value}
-  : forall (f : Value -> Value) (bag : t Value) bag' k v, 
-      InA (@eq_key_elt _) (k,v) (List.map (fun kv => (fst kv, f (snd kv))) (elements bag))
-      -> MapsTo k v
-           (fold (fun k bag'' r' => add k (f bag'') r') bag bag').
-  Proof.
-    intros; rewrite fold_1 in *; revert k v bag' H;
-    generalize (elements_3w bag); induction (elements bag); 
-    intros; inversion H0; inversion H; subst; simpl in *; eauto.
-    destruct H2; simpl in *; subst; rewrite H1.
-    apply FMap_fold_add_MapsTo_NIn; eauto.
-    unfold not, eq_key in *; intros; apply H6; revert H2; clear; 
-    induction l; simpl in *; intros; inversion H2; subst; eauto.
-    apply add_1; reflexivity.
-  Qed.
+    Lemma FMap_fold_add_MapsTo_In {Value}
+    : forall (f : Value -> Value) (bag : t Value) bag' k v,
+        InA (@eq_key_elt _) (k,v) (List.map (fun kv => (fst kv, f (snd kv))) (elements bag))
+        -> MapsTo k v
+                  (fold (fun k bag'' r' => add k (f bag'') r') bag bag').
+    Proof.
+      intros; rewrite fold_1 in *; revert k v bag' H;
+      generalize (elements_3w bag); induction (elements bag);
+      intros; inversion H0; inversion H; subst; simpl in *; eauto.
+      destruct H2; simpl in *; subst; rewrite H1.
+      apply FMap_fold_add_MapsTo_NIn; eauto.
+      unfold not, eq_key in *; intros; apply H6; revert H2; clear;
+      induction l; simpl in *; intros; inversion H2; subst; eauto.
+      apply add_1; reflexivity.
+    Qed.
 
-  Lemma FMap_Insert_fold_add_MapsTo {Value}
-  : forall (f : Value -> Value) (bag : t Value) bag' k v, 
-      MapsTo k v
-           (fold (fun k bag'' r' => add k (f bag'') r') bag bag') -> 
-      MapsTo k v bag' \/
-      InA (@eq_key_elt _) (k,v) (List.map (fun kv => (fst kv, f (snd kv))) (elements bag)).
-  Proof.
-    intros; rewrite fold_1 in *; revert bag' H;
-    induction (elements bag); simpl in *; eauto; intros.
-    apply IHl in H; intuition.
-    apply add_mapsto_iff in H0; intuition; subst.
-    right; constructor; split; eauto.
-  Qed.
+    Lemma FMap_Insert_fold_add_MapsTo {Value}
+    : forall (f : Value -> Value) (bag : t Value) bag' k v,
+        MapsTo k v
+               (fold (fun k bag'' r' => add k (f bag'') r') bag bag') ->
+        MapsTo k v bag' \/
+        InA (@eq_key_elt _) (k,v) (List.map (fun kv => (fst kv, f (snd kv))) (elements bag)).
+    Proof.
+      intros; rewrite fold_1 in *; revert bag' H;
+      induction (elements bag); simpl in *; eauto; intros.
+      apply IHl in H; intuition.
+      apply add_mapsto_iff in H0; intuition; subst.
+      right; constructor; split; eauto.
+    Qed.
 
-  Lemma InA_Map {A B} eqB
-  : forall (f : A -> B) (b : B) (l : list A), 
-      InA eqB b (List.map f l) <-> 
-      exists a, eqB b (f a) /\ List.In a l.
-  Proof.
-    split; induction l; simpl; intros; inversion H; subst; 
-    eauto. destruct (IHl H1) as [a' [In_a eq_b]]; eauto.
-    intuition.
-    intuition; subst.
-    constructor; eauto.
-    constructor 2; eauto.
-  Qed.
-
-  Lemma FMap_Insert_fold_add_map_eq {Value}
-  : forall (f : Value -> Value) (bag : t Value), 
-      Equal
-           (fold (fun k bag'' r' => add k (f bag'') r') bag (empty _))
-           (map f bag).
-  Proof.
-    unfold Equal.
-    intros; case_eq (find y
-                          (fold
-                             (fun (k : key) (bag'' : Value) (r' : t Value) => add k (f bag'') r')
-                             bag (empty Value)));
-    intros; case_eq (find y (map f bag)); intros; eauto.
-    - apply find_2 in H; apply find_2 in H0.
-      apply FMap_Insert_fold_add_MapsTo in H; destruct H.
-      elimtype False; apply empty_mapsto_iff in H; eauto.
-      apply map_mapsto_iff in H0; destruct H0 as [a [eq_a MapsTo_y]]; subst.
-      generalize (elements_3w bag); apply elements_1 in MapsTo_y; 
-      induction MapsTo_y; intros.
-      + inversion H1; subst; destruct H0; simpl in *; subst.
-        inversion H; subst;
-        [destruct H3; simpl in *; subst; eauto 
-        | elimtype False; apply H4; revert H0 H3; clear; induction l; 
-          intros; inversion H3; subst; unfold eq_key in *].
-        destruct H1; simpl in *; subst; constructor; eauto.
-        constructor 2; eauto.
-      + inversion H0; subst; eapply IHMapsTo_y; eauto.
-        inversion H; subst; eauto.
-        destruct H2; simpl in *; subst.
-        elimtype False; apply H3; revert H1 MapsTo_y; clear; induction l;
-        intros; inversion MapsTo_y; subst; unfold eq_key in *.
-        destruct H0; simpl in *; subst; constructor; eauto.
-        constructor 2; eauto.
-    - apply find_2 in H; apply FMap_Insert_fold_add_MapsTo in H; destruct H.
-      elimtype False; apply empty_mapsto_iff in H; eauto.
-      apply InA_Map in H; destruct H as [[k v'] [eq_k In_k]]; simpl in *.
-      destruct eq_k; simpl in *; rewrite H in H0.
-      apply not_find_in_iff in H0; elimtype False; eapply H0.
-      apply map_in_iff; exists v'; apply elements_2.
-      apply InA_alt; eexists; repeat split; eauto.
-    - apply find_2 in H0; apply not_find_in_iff in H.
-      apply map_mapsto_iff in H0; destruct H0 as [k [k_eq MapsTo_k]]; subst.
-      elimtype False; apply H.
-      econstructor 1 with (x := f k); apply FMap_fold_add_MapsTo_In.
-      apply elements_1 in MapsTo_k; revert MapsTo_k; clear;
-      intro; induction MapsTo_k; simpl.
-      repeat constructor; destruct H; simpl in *; subst; eauto.
+    Lemma InA_Map {A B} eqB
+    : forall (f : A -> B) (b : B) (l : list A),
+        InA eqB b (List.map f l) <->
+        exists a, eqB b (f a) /\ List.In a l.
+    Proof.
+      split; induction l; simpl; intros; inversion H; subst;
+      eauto. destruct (IHl H1) as [a' [In_a eq_b]]; eauto.
+      intuition.
+      intuition; subst.
+      constructor; eauto.
       constructor 2; eauto.
-  Qed.
+    Qed.
 
-  Definition IndexedBag_bdelete'
-             (container: IndexedBag)
-             (key_searchterm: (option TKey) * TBagSearchTerm)
-  : (list TItem) * (t TBag) :=
-    let (key_option, search_term) := key_searchterm in
-    match key_option with
-      | Some k => (match find k (ifmap container) with
-                      | Some bag => @benumerate _ _ _ _ bags_bag bag
-                      | None => nil
-                   end, @remove TBag k (ifmap container))
-      | None => fold (fun k bag (res : (list TItem) * (t TBag)) =>
-                        match @bdelete _ _ _ _ bags_bag bag search_term with 
-                          | (d, r) => let (d', r') := res in
-                                      (d ++ d', add k r r')
-                        end) (ifmap container) ([], empty TBag)
-    end.
-  
-  Lemma In_partition {A} 
-  : forall f (l : list A) a, 
-      List.In a l <-> (List.In a (fst (List.partition f l))
-                       \/ List.In a (snd (List.partition f l))).
-  Proof.
-    split; induction l; simpl; intros; intuition; simpl; subst; 
-    first [destruct (f a0); destruct (List.partition f l); simpl in *; intuition
-          | destruct (f a); destruct (List.partition f l); simpl; intuition].
-  Qed.
-    
-  Lemma IndexedBag_bdelete_consistent
-        (container: IndexedBag)
-        (key_searchterm: (option TKey) * TBagSearchTerm)
-  : IndexedTreeConsistency (snd (IndexedBag_bdelete' container key_searchterm)).
-  Proof.
-    intros; destruct key_searchterm; destruct o; simpl in *;
-    unfold IndexedTreeConsistency; intros.
-    + apply remove_3 in H; eapply iconsistency; eauto.
-    + destruct container as [bag' WF_bag']; simpl in *.
-      assert (forall l, 
-                snd
-                  (fold_left
-                     (fun (a : list TItem * t TBag) (p : key * TBag) =>
-                        let (d, r) := bdelete (snd p) t0 in
-                        let (d', r') := a in (d ++ d', add (fst p) r r'))
-                     (elements bag') l)
-                = fold_left
-                            (fun (a : t TBag) (p : key * TBag) =>
-                               add (fst p) (snd (bdelete (snd p) t0))a) 
-                            (elements bag') (snd l)).
-      { induction (elements bag'); simpl in *; eauto.
-        intros; rewrite IHl; destruct l0; 
-        destruct (bdelete (snd a) t0); simpl; reflexivity. }
-      assert (MapsTo key0 bag 
-                     (fold
-                        (fun (k : key) (bag0 : TBag) (r' : t TBag) =>
-                           add k (snd (bdelete bag0 t0)) r') bag'
-                        (empty TBag)))
-      by (rewrite fold_1, H1 in H; simpl in H;  rewrite fold_1; eauto); clear H H1.
-      rewrite FMap_Insert_fold_add_map_eq in H2.
-      apply map_mapsto_iff in H2; destruct H2 as [k [k_eq MapsTo_k]]; subst.
-      eapply WF_bag'; eauto.
-      destruct (bdelete_correct k t0).
-      eapply In_partition; right; eapply Permutation_in; eauto.
-  Qed.
+    Lemma FMap_Insert_fold_add_map_eq {Value}
+    : forall (f : Value -> Value) (bag : t Value),
+        Equal
+          (fold (fun k bag'' r' => add k (f bag'') r') bag (empty _))
+          (map f bag).
+    Proof.
+      unfold Equal.
+      intros; case_eq (find y
+                            (fold
+                               (fun (k : key) (bag'' : Value) (r' : t Value) => add k (f bag'') r')
+                               bag (empty Value)));
+      intros; case_eq (find y (map f bag)); intros; eauto.
+      - apply find_2 in H; apply find_2 in H0.
+        apply FMap_Insert_fold_add_MapsTo in H; destruct H.
+        elimtype False; apply empty_mapsto_iff in H; eauto.
+        apply map_mapsto_iff in H0; destruct H0 as [a [eq_a MapsTo_y]]; subst.
+        generalize (elements_3w bag); apply elements_1 in MapsTo_y;
+        induction MapsTo_y; intros.
+        + inversion H1; subst; destruct H0; simpl in *; subst.
+          inversion H; subst;
+          [destruct H3; simpl in *; subst; eauto
+          | elimtype False; apply H4; revert H0 H3; clear; induction l;
+            intros; inversion H3; subst; unfold eq_key in *].
+          destruct H1; simpl in *; subst; constructor; eauto.
+          constructor 2; eauto.
+        + inversion H0; subst; eapply IHMapsTo_y; eauto.
+          inversion H; subst; eauto.
+          destruct H2; simpl in *; subst.
+          elimtype False; apply H3; revert H1 MapsTo_y; clear; induction l;
+          intros; inversion MapsTo_y; subst; unfold eq_key in *.
+          destruct H0; simpl in *; subst; constructor; eauto.
+          constructor 2; eauto.
+      - apply find_2 in H; apply FMap_Insert_fold_add_MapsTo in H; destruct H.
+        elimtype False; apply empty_mapsto_iff in H; eauto.
+        apply InA_Map in H; destruct H as [[k v'] [eq_k In_k]]; simpl in *.
+        destruct eq_k; simpl in *; rewrite H in H0.
+        apply not_find_in_iff in H0; elimtype False; eapply H0.
+        apply map_in_iff; exists v'; apply elements_2.
+        apply InA_alt; eexists; repeat split; eauto.
+      - apply find_2 in H0; apply not_find_in_iff in H.
+        apply map_mapsto_iff in H0; destruct H0 as [k [k_eq MapsTo_k]]; subst.
+        elimtype False; apply H.
+        econstructor 1 with (x := f k); apply FMap_fold_add_MapsTo_In.
+        apply elements_1 in MapsTo_k; revert MapsTo_k; clear;
+        intro; induction MapsTo_k; simpl.
+        repeat constructor; destruct H; simpl in *; subst; eauto.
+        constructor 2; eauto.
+    Qed.
 
+    Definition IndexedBag_bdelete'
+               (container: IndexedBag)
+               (key_searchterm: (option TKey) * TBagSearchTerm)
+    : (list TItem) * (t TBag) :=
+      let (key_option, search_term) := key_searchterm in
+      match key_option with
+        | Some k => (match find k (ifmap container) with
+                       | Some bag => benumerate (Bag := KeyPreserving_bag) bag
+                       | None => nil
+                     end, @remove TBag k (ifmap container))
+        | None => fold (fun k bag (res : (list TItem) * (t TBag)) =>
+                          match bdelete (Bag := KeyPreserving_bag) bag search_term with
+                            | (d, r) => let (d', r') := res in
+                                        (d ++ d', add k r r')
+                          end) (ifmap container) ([], empty TBag)
+      end.
 
-  Lemma MapDelete_IndexedBag_consistent
-        (container : t TBag)
-        (search_term: TBagSearchTerm)
-  : IndexedTreeConsistency container
-    -> IndexedTreeConsistency (map (fun bag : TBag => bdelete bag search_term) container).
-  Proof.
-    unfold IndexedTreeConsistency; intros.
-    assert (In key0 container) by (eapply map_2; econstructor; eauto).
-    destruct H2.
-    eapply H; eauto.
-    pose proof (map_1 ((fun bag : TBag => bdelete bag search_term)) H2).
-    apply find_1 in H3; apply find_1 in H0.
-    rewrite H0 in H3; injection H3; intros; subst.
-    assert (List.In item (snd (List.partition (bfind_matcher search_term) (benumerate x)))).
-    { eapply Permutation_in. eapply bdelete_correct. eauto. }
+    Lemma In_partition {A}
+    : forall f (l : list A) a,
+        List.In a l <-> (List.In a (fst (List.partition f l))
+                         \/ List.In a (snd (List.partition f l))).
+    Proof.
+      split; induction l; simpl; intros; intuition; simpl; subst;
+      first [destruct (f a0); destruct (List.partition f l); simpl in *; intuition
+            | destruct (f a); destruct (List.partition f l); simpl; intuition].
+    Qed.
 
-eapply
+    Lemma In_partition_matched {A}
+    : forall f (l : list A) a,
+        List.In a (fst (List.partition f l)) ->
+        f a = true.
+    Proof.
+      induction l; simpl; intros; intuition; simpl; subst; eauto.
+      case_eq (f a); destruct (List.partition f l); simpl; intuition;
+      rewrite H0 in H; eauto; inversion H; subst; eauto.
+    Qed.
 
+    Lemma In_partition_unmatched {A}
+    : forall f (l : list A) a,
+        List.In a (snd (List.partition f l)) ->
+        f a = false.
+    Proof.
+      induction l; simpl; intros; intuition; simpl; subst; eauto.
+      case_eq (f a); destruct (List.partition f l); simpl; intuition;
+      rewrite H0 in H; eauto; inversion H; subst; eauto.
+    Qed.
 
-    apply find_1 in H0; rewrite map_o in H0.
-    unfold option_map in *.
-    destruct (find key0 container).
-    eapply H with (bag := t0). (* with (bag := bdelete bag search_term). *)
-    apply find_2.
+    Lemma IndexedBag_bdelete_consistent
+          (container: IndexedBag)
+          (key_searchterm: (option TKey) * TBagSearchTerm)
+    : IndexedTreeConsistency (snd (IndexedBag_bdelete' container key_searchterm)).
+    Proof.
+      intros; destruct key_searchterm; destruct o; simpl in *;
+      unfold IndexedTreeConsistency; intros.
+      - apply remove_3 in H; eapply iconsistency; eauto.
+      - destruct container as [bag' WF_bag']; simpl in *.
+        assert (forall l,
+                  snd
+                    (fold_left
+                       (fun (a : list TItem * t TBag) (p : key * TBag) =>
+                          let (d, r) := bdelete (snd p) t0 in
+                          let (d', r') := a in (d ++ d', add (fst p) r r'))
+                       (elements bag') l)
+                  = fold_left
+                      (fun (a : t TBag) (p : key * TBag) =>
+                         add (fst p) (snd (bdelete (snd p) t0))a)
+                      (elements bag') (snd l)).
+        { induction (elements bag'); simpl in *; eauto.
+          intros; rewrite IHl; destruct l0;
+          destruct (bdelete (snd a) t0); simpl; reflexivity. }
+        assert (MapsTo key0 bag
+                       (fold
+                          (fun (k : key) (bag0 : TBag) (r' : t TBag) =>
+                             add k (snd (bdelete bag0 t0)) r') bag'
+                          (empty TBag)))
+          by (rewrite fold_1, H1 in H; simpl in H;  rewrite fold_1; eauto); clear H H1.
+        rewrite FMap_Insert_fold_add_map_eq in H2.
+        apply map_mapsto_iff in H2; destruct H2 as [k [k_eq MapsTo_k]]; subst.
+        eapply WF_bag'; eauto.
+        destruct (bdelete_correct k t0).
+        eapply In_partition; right; eapply Permutation_in; eauto.
+    Defined.
 
+    Definition IndexedBag_bdelete
+               (container: IndexedBag)
+               (key_searchterm: (option TKey) * TBagSearchTerm)
+    : ((list TItem) * IndexedBag) :=
+      match IndexedBag_bdelete' container key_searchterm as l
+            return IndexedTreeConsistency (snd l) -> ((list TItem) * IndexedBag) with
+        | (deleted, container') =>
+          fun i => (deleted, {|ifmap := container';
+                               iconsistency := i |})
+      end (IndexedBag_bdelete_consistent container key_searchterm).
 
+    Definition IndexedBag_bupdate'
+               (container: IndexedBag)
+               (key_searchterm: (option TKey) * TBagSearchTerm)
+               (updateTerm : TBagUpdateTerm)
+    : (t TBag) :=
+      let (key_option, search_term) := key_searchterm in
+      match key_option with
+        | Some k => match find k (ifmap container) with
+                      | Some bag => add k (bupdate bag search_term updateTerm) (ifmap container)
+                      | None => (ifmap container)
+                    end
+        | None => map (fun bag => bupdate bag search_term updateTerm) (ifmap container)
+      end.
 
-    rewrite map_o in H
-    assert (In key0
-               (map (fun bag0 : TBag => bdelete bag0 search_term) container))
-      by (econstructor; eauto).
-    apply map_2 in H2.
-    destruct H2.
+    Lemma IndexedBag_bupdate'_consistent
+          (container : IndexedBag)
+          (key_searchterm: (option TKey) * TBagSearchTerm)
+          (updateTerm : TBagUpdateTerm)
+    : IndexedTreeConsistency (IndexedBag_bupdate' container key_searchterm updateTerm).
+    Proof.
+      intros; destruct key_searchterm; destruct o; simpl in *.
+      - case_eq (find t1 (ifmap container)); intros; eauto using iconsistency.
+        unfold IndexedTreeConsistency; intros.
+        apply add_mapsto_iff in H0; intuition.
+        + pose proof (bupdate_correct t2 t0 updateTerm).
+          rewrite <- H3 in H1.
+          apply find_2 in H; rewrite <- H0.
+          pose proof (Permutation_in _ H2 H1) as H4;
+            apply in_app_or in H4; destruct H4.
+          * pose proof ((proj2 (In_partition _ _ _)) (or_intror H4));
+            eapply iconsistency; eauto.
+          * apply in_map_iff in H4; destruct H4 as [item' [item'_eq In_item']].
+            pose proof (iconsistency _ _ _ H _
+                                     ((proj2 (In_partition _ _ _)) (or_introl In_item'))).
+            rewrite <- H4.
+            rewrite <- item'_eq.
+            eapply KeyPreserving_Proof; eauto using In_partition_matched.
+        + eapply iconsistency; eauto.
+      - unfold IndexedTreeConsistency; intros.
+        apply map_mapsto_iff in H;
+          destruct H as [bag' [bag'_eq MapsTo_key0]]; subst.
+        pose proof (bupdate_correct bag' t0 updateTerm).
+        pose proof (Permutation_in _ H H0) as H4;
+          apply in_app_or in H4; destruct H4.
+        + pose proof ((proj2 (In_partition _ _ _)) (or_intror H1));
+          eapply iconsistency; eauto.
+        + apply in_map_iff in H1; destruct H1 as [item' [item'_eq In_item']].
+          pose proof (iconsistency _ _ _ MapsTo_key0 _
+                                   ((proj2 (In_partition _ _ _)) (or_introl In_item'))).
+          rewrite <- H1.
+          rewrite <- item'_eq.
+          eapply KeyPreserving_Proof; eauto using In_partition_matched.
+    Defined.
 
+    Definition IndexedBag_bupdate
+               (container: IndexedBag)
+               (key_searchterm: (option TKey) * TBagSearchTerm)
+               (updateTerm : TBagUpdateTerm)
+    : IndexedBag :=
+      {| ifmap := IndexedBag_bupdate' container key_searchterm updateTerm;
+         iconsistency := IndexedBag_bupdate'_consistent container key_searchterm updateTerm |}.
 
+    Definition IndexedBag_bcount
+               (container: IndexedBag)
+               (key_searchterm: (option TKey) * TBagSearchTerm) :=
+      let (key_option, search_term) := key_searchterm in
+      match key_option with
+        | Some k =>
+          match find k (ifmap container) with
+            | Some bag => bcount (Bag := KeyPreserving_bag) bag search_term
+            | None     => 0
+          end
+        | None   =>
+          fold (fun _ bag acc => acc + bcount (Bag := KeyPreserving_bag) bag search_term)
+               (ifmap container) 0
+      end.
 
+    Lemma indexed_bag_insert_consistent :
+      forall (container: IndexedBag)
+             (item: TItem),
+        let k := projection item in
+        let fmap := ifmap container in
+        let bag := FindWithDefault k bempty fmap in
+        IndexedTreeConsistency (add k (binsert bag item) fmap).
+    Proof.
+      intros.
 
-  Lemma MapDelete_IndexedBag_consistent
-        {TBag TItem TBagSearchTerm: Type}
-        {bags_bag: Bag TBag TItem TBagSearchTerm}
-        (projection: TItem -> TKey)
-        (container: @IndexedBag TBag TItem TBagSearchTerm bags_bag projection)
-        (search_term: TBagSearchTerm)
-  : IndexedTreeConsistency projection
-                           (map (fun bag : TBag => bdelete bag search_term) (ifmap container)).
-  Proof.
-    unfold IndexedTreeConsistency; intros.
-    destruct container; simpl in *.
-    eapply iconsistency; eauto.
-    Check
-    apply find_mapsto_iff in H.
-    destruct container; simpl in *.
-    eapply iconsistency; eauto.
-    eapply find_2.
+      intros k' bag' maps_to item'.
 
-    eapply iconsisitency.
-    Print find.
+      rewrite add_mapsto_iff in maps_to;
+        destruct maps_to as [(is_eq & refreshed) | (neq & maps_to)];
+        subst.
 
-    destruct (find key0 (ifmap container)).
-    simpl in H.
-unfold IndexedTreeConsistency; intros.
+      rewrite (binsert_enumerate_weak item' item bag).
+      intro H; destruct H.
+      apply ((iconsistency container) k' bag); trivial.
 
+      rewrite <- is_eq.
+      unfold bag in *.
 
+      unfold fmap in *.
+      destruct (FindWithDefault_dec k (bempty (Bag := KeyPreserving_bag)) (ifmap container))
+        as [ [bag' (mapsto & equality)] | (not_found & equality) ];
+        rewrite equality in *; clear equality.
 
+      subst; trivial.
+      exfalso; apply (benumerate_empty) in H; trivial.
 
+      subst.
+      unfold k in *.
+      trivial.
 
-        flatten (List.map (fun bag =>  @bfind _ _ _ bags_bag bag search_term) (Values (ifmap container)))
-    end.
+      apply ((iconsistency container) k' bag' maps_to item').
+    Qed.
 
-  Definition IndexedBag_bcount
-             {TBag TItem TBagSearchTerm: Type}
-             {bags_bag: Bag TBag TItem TBagSearchTerm}
-             (projection: TItem -> TKey)
-             (container: @IndexedBag TBag TItem TBagSearchTerm bags_bag projection)
-             (key_searchterm: (option TKey) * TBagSearchTerm) :=
-    let (key_option, search_term) := key_searchterm in
-    match key_option with
-      | Some k =>
-        match find k (ifmap container) with
-          | Some bag => @bcount _ _ _ bags_bag bag search_term
-          | None     => 0
-        end
-      | None   =>
-        fold (fun _ bag acc => acc + @bcount _ _ _ bags_bag bag search_term) (ifmap container) 0
-    end.
-
-  Lemma indexed_bag_insert_consistent :
-    forall {TBag TItem TBagSearchTerm: Type}
-           {bags_bag: Bag TBag TItem TBagSearchTerm}
-           {projection: TItem -> TKey}
-           (container: @IndexedBag TBag TItem TBagSearchTerm bags_bag projection)
-           (item: TItem),
+    Definition IndexedBag_binsert
+               (container: IndexedBag)
+               (item: TItem) : IndexedBag :=
       let k := projection item in
       let fmap := ifmap container in
       let bag := FindWithDefault k bempty fmap in
-      IndexedTreeConsistency projection (add k (binsert bag item) fmap).
-  Proof.
-    intros.
+      {|
+        ifmap := add k (binsert bag item) fmap;
+        iconsistency := indexed_bag_insert_consistent container item
+      |}.
 
-    intros k' bag' maps_to item'.
+    Add Parametric Morphism {A} :
+      (@cons A)
+        with signature (eq ==> eq ==> eq)
+          as cons_eq_eq_eq_morphism.
+    Proof.
+      trivial.
+    Qed.
 
-    rewrite add_mapsto_iff in maps_to;
-      destruct maps_to as [(is_eq & refreshed) | (neq & maps_to)];
-      subst.
+    Lemma elements_fold_eq :
+      forall {TValues} (m: t TValues),
+        (elements m) =
+        (rev (fold (fun key val acc => cons (key, val) acc) m [])).
+    Proof.
+      intros.
+      rewrite fold_1.
 
-    rewrite (binsert_enumerate_weak item' item bag).
-    intro H; destruct H.
-    apply ((iconsistency container) k' bag); trivial.
+      setoid_rewrite <- surjective_pairing.
+      setoid_rewrite fold_left_id.
+      rewrite rev_involutive; reflexivity.
+    Qed.
 
-    rewrite <- is_eq.
-    unfold bag in *.
+    Lemma elements_fold_perm :
+      forall {TValues} (m: t TValues),
+        Permutation
+          (elements m)
+          (fold (fun key val acc => cons (key, val) acc) m []).
+    Proof.
+      intros.
+      rewrite fold_1.
 
-    unfold fmap in *.
-    destruct (FindWithDefault_dec k (@bempty _ _ _ bags_bag) (ifmap container))
-      as [ [bag' (mapsto & equality)] | (not_found & equality) ];
-      rewrite equality in *; clear equality.
+      setoid_rewrite <- surjective_pairing.
+      setoid_rewrite fold_left_id.
+      apply Permutation_rev.
+    Qed.
 
-    subst; trivial.
-    exfalso; apply (@benumerate_empty _ _ _ bags_bag) in H; trivial.
+    Lemma fold_right_map :
+      forall {A B} f seq,
+        @List.fold_right (list B) A (fun b a => f b :: a) [] seq = List.map f seq.
+    Proof.
+      intros; induction seq; simpl; try rewrite IHseq; reflexivity.
+    Qed.
 
-    subst.
-    unfold k in *.
-    trivial.
+    Lemma fold_left_map :
+      forall {A B} f seq,
+        @List.fold_left (list B) A (fun a b => f b :: a) seq [] = List.map f (rev seq).
+    Proof.
+      intros; rewrite <- fold_left_rev_right; apply fold_right_map.
+    Qed.
 
-    apply ((iconsistency container) k' bag' maps_to item').
-  Qed.
+    Lemma Values_fold_perm :
+      forall {TValues} (m: t TValues),
+        Permutation
+          (Values m)
+          (fold (fun key val acc => cons val acc) m []).
+    Proof.
+      intros.
+      rewrite fold_1.
 
-  Definition IndexedBag_binsert
-             {TBag TItem TBagSearchTerm: Type}
-             {bags_bag: Bag TBag TItem TBagSearchTerm}
-             (projection: TItem -> TKey)
-             (container: @IndexedBag TBag TItem TBagSearchTerm bags_bag projection)
-             (item: TItem) : @IndexedBag TBag TItem TBagSearchTerm bags_bag projection :=
-    let k := projection item in
-    let fmap := ifmap container in
-    let bag := FindWithDefault k bempty fmap in
-    {|
-      ifmap := add k (binsert bag item) fmap;
-      iconsistency := indexed_bag_insert_consistent container item
-    |}.
+      rewrite fold_left_map.
+      unfold Values.
 
-  Add Parametric Morphism {A} :
-    (@cons A)
-      with signature (eq ==> eq ==> eq)
-        as cons_eq_eq_eq_morphism.
-  Proof.
-    trivial.
-  Qed.
+      rewrite map_rev.
+      apply Permutation_rev.
+    Qed.
 
-  Lemma elements_fold_eq :
-    forall {TValues} (m: t TValues),
-      (elements m) =
-      (rev (fold (fun key val acc => cons (key, val) acc) m [])).
-  Proof.
-    intros.
-    rewrite fold_1.
+    Lemma Values_fold_eq :
+      forall {TValues} (m: t TValues),
+        (Values m) =
+        (rev (fold (fun key val acc => cons val acc) m [])).
+    Proof.
+      intros.
+      rewrite fold_1.
 
-    setoid_rewrite <- surjective_pairing.
-    setoid_rewrite fold_left_id.
-    rewrite rev_involutive; reflexivity.
-  Qed.
+      rewrite fold_left_map.
+      unfold Values.
 
-  Lemma elements_fold_perm :
-    forall {TValues} (m: t TValues),
-      Permutation
-        (elements m)
-        (fold (fun key val acc => cons (key, val) acc) m []).
-  Proof.
-    intros.
-    rewrite fold_1.
-
-    setoid_rewrite <- surjective_pairing.
-    setoid_rewrite fold_left_id.
-    apply Permutation_rev.
-  Qed.
-
-  Lemma fold_right_map :
-    forall {A B} f seq,
-      @List.fold_right (list B) A (fun b a => f b :: a) [] seq = List.map f seq.
-  Proof.
-    intros; induction seq; simpl; try rewrite IHseq; reflexivity.
-  Qed.
-
-  Lemma fold_left_map :
-    forall {A B} f seq,
-      @List.fold_left (list B) A (fun a b => f b :: a) seq [] = List.map f (rev seq).
-  Proof.
-    intros; rewrite <- fold_left_rev_right; apply fold_right_map.
-  Qed.
-
-  Lemma Values_fold_perm :
-    forall {TValues} (m: t TValues),
-      Permutation
-        (Values m)
-        (fold (fun key val acc => cons val acc) m []).
-  Proof.
-    intros.
-    rewrite fold_1.
-
-    rewrite fold_left_map.
-    unfold Values.
-
-    rewrite map_rev.
-    apply Permutation_rev.
-  Qed.
-
-  Lemma Values_fold_eq :
-    forall {TValues} (m: t TValues),
-      (Values m) =
-      (rev (fold (fun key val acc => cons val acc) m [])).
-  Proof.
-    intros.
-    rewrite fold_1.
-
-    rewrite fold_left_map.
-    unfold Values.
-
-    rewrite map_rev.
-    rewrite rev_involutive; reflexivity.
-  Qed.
+      rewrite map_rev.
+      rewrite rev_involutive; reflexivity.
+    Qed.
 
 
-  Lemma map_fold :
-    forall {A B TValue} f g m init,
-      (@List.map A B g
-                 (fold
-                    (fun k (v: TValue) acc =>
-                       f k v :: acc) m init)) =
-      (fold (fun k v acc => g (f k v) :: acc) m (List.map g init)).
-  Proof.
-    intros until m; setoid_rewrite fold_1.
-    setoid_rewrite <- fold_left_rev_right; simpl.
-    induction (elements m) as [ | ? ? IH ]; simpl; trivial.
-    setoid_rewrite fold_right_app.
-    setoid_rewrite IH; simpl.
-    reflexivity.
-  Qed.
+    Lemma map_fold :
+      forall {A B TValue} f g m init,
+        (@List.map A B g
+                   (fold
+                      (fun k (v: TValue) acc =>
+                         f k v :: acc) m init)) =
+        (fold (fun k v acc => g (f k v) :: acc) m (List.map g init)).
+    Proof.
+      intros until m; setoid_rewrite fold_1.
+      setoid_rewrite <- fold_left_rev_right; simpl.
+      induction (elements m) as [ | ? ? IH ]; simpl; trivial.
+      setoid_rewrite fold_right_app.
+      setoid_rewrite IH; simpl.
+      reflexivity.
+    Qed.
 
-  Lemma values_add_not_in :
-    forall {TBag: Type} (m: t TBag),
-    forall k v,
-      ~ In k m ->
-      Permutation
-        (Values (add k v m))
-        (v :: Values m).
-  Proof.
-    intros.
-    unfold Values.
-    rewrite elements_fold_eq.
+    Lemma values_add_not_in :
+      forall (m: t TBag),
+      forall k v,
+        ~ In k m ->
+        Permutation
+          (Values (add k v m))
+          (v :: Values m).
+    Proof.
+      intros.
+      unfold Values.
+      rewrite elements_fold_eq.
 
-    rewrite map_rev.
-    rewrite map_fold; simpl.
-    rewrite (fold_add (eqA := @Permutation _)).
-    rewrite fold_1.
-    rewrite fold_left_map.
-    simpl.
+      rewrite map_rev.
+      rewrite map_fold; simpl.
+      rewrite (fold_add (eqA := @Permutation _)).
+      rewrite fold_1.
+      rewrite fold_left_map.
+      simpl.
 
-    rewrite map_rev.
-    rewrite rev_involutive.
+      rewrite map_rev.
+      rewrite rev_involutive.
 
-    etransitivity.
-    apply Permutation_app_comm.
-    simpl; reflexivity.
+      etransitivity.
+      apply Permutation_app_comm.
+      simpl; reflexivity.
 
-    apply Permutation_Equivalence.
+      apply Permutation_Equivalence.
 
-    unfold Proper, respectful; intros; simpl;
-    subst; apply Permutation_cons; assumption.
+      unfold Proper, respectful; intros; simpl;
+      subst; apply Permutation_cons; assumption.
 
-    unfold transpose_neqkey; intros; simpl;
-    constructor.
+      unfold transpose_neqkey; intros; simpl;
+      constructor.
 
-    assumption.
-  Qed.
+      assumption.
+    Qed.
 
 
-  Definition KeyBasedPartitioningFunction TBag reference :=
-    fun key (_: TBag) => if E.eq_dec key reference then true else false.
+    Definition KeyBasedPartitioningFunction TBag reference :=
+      fun key (_: TBag) => if E.eq_dec key reference then true else false.
 
-  Lemma KeyBasedPartitioningFunction_Proper :
-    forall TBag reference,
-      Proper (E.eq ==> eq ==> eq) (KeyBasedPartitioningFunction TBag reference).
-  Proof.
-    intros;
-    unfold KeyBasedPartitioningFunction, Proper, respectful; intros x y E_eq **; subst;
-    destruct (F.eq_dec x _), (F.eq_dec y _); rewrite E_eq in *; intuition.
-  Qed.
+    Lemma KeyBasedPartitioningFunction_Proper :
+      forall TBag reference,
+        Proper (E.eq ==> eq ==> eq) (KeyBasedPartitioningFunction TBag reference).
+    Proof.
+      intros;
+      unfold KeyBasedPartitioningFunction, Proper, respectful; intros x y E_eq **; subst;
+      destruct (F.eq_dec x _), (F.eq_dec y _); rewrite E_eq in *; intuition.
+    Qed.
 
-  Lemma eq_dec_refl :
-    forall x,
-      (if E.eq_dec x x then true else false) = true.
-  Proof.
-    intros; destruct (E.eq_dec _ _); eauto using E.eq_refl.
-  Qed.
+    Lemma eq_dec_refl :
+      forall x,
+        (if E.eq_dec x x then true else false) = true.
+    Proof.
+      intros; destruct (E.eq_dec _ _); eauto using E.eq_refl.
+    Qed.
 
-  Lemma eq_dec_comm :
-    forall x y,
-      (if E.eq_dec x y then true else false) = (if E.eq_dec y x then true else false).
-  Proof.
-    intros; destruct (E.eq_dec x y), (E.eq_dec y x); intuition.
-  Qed.
+    Lemma eq_dec_comm :
+      forall x y,
+        (if E.eq_dec x y then true else false) = (if E.eq_dec y x then true else false).
+    Proof.
+      intros; destruct (E.eq_dec x y), (E.eq_dec y x); intuition.
+    Qed.
 
-  Lemma KeyBasedPartitioningFunction_eq_true :
-    forall TValue k k' v,
-      E.eq k k' <->
-      KeyBasedPartitioningFunction TValue k k' v = true.
-  Proof.
-    intros; unfold KeyBasedPartitioningFunction; destruct (E.eq_dec _ _); intuition.
-  Qed.
+    Lemma KeyBasedPartitioningFunction_eq_true :
+      forall TValue k k' v,
+        E.eq k k' <->
+        KeyBasedPartitioningFunction TValue k k' v = true.
+    Proof.
+      intros; unfold KeyBasedPartitioningFunction; destruct (E.eq_dec _ _); intuition.
+    Qed.
 
-  Lemma KeyBasedPartitioningFunction_eq_false :
-    forall TValue k k' v,
-      ~ E.eq k k' <->
-      KeyBasedPartitioningFunction TValue k k' v = false.
-  Proof.
-    intros; unfold KeyBasedPartitioningFunction; destruct (E.eq_dec _ _); intuition.
-  Qed.
+    Lemma KeyBasedPartitioningFunction_eq_false :
+      forall TValue k k' v,
+        ~ E.eq k k' <->
+        KeyBasedPartitioningFunction TValue k k' v = false.
+    Proof.
+      intros; unfold KeyBasedPartitioningFunction; destruct (E.eq_dec _ _); intuition.
+    Qed.
 
-  Lemma KeyBasedPartitioningFunction_refl :
-    forall TValue k k' v,
-      KeyBasedPartitioningFunction TValue k k' v = KeyBasedPartitioningFunction TValue k' k v.
-  Proof.
-    intros; unfold KeyBasedPartitioningFunction; rewrite eq_dec_comm; reflexivity.
-  Qed.
+    Lemma KeyBasedPartitioningFunction_refl :
+      forall TValue k k' v,
+        KeyBasedPartitioningFunction TValue k k' v = KeyBasedPartitioningFunction TValue k' k v.
+    Proof.
+      intros; unfold KeyBasedPartitioningFunction; rewrite eq_dec_comm; reflexivity.
+    Qed.
 
-  (*
+    (*
     Lemma fold_over_add :
       forall {TValue} k v v' (m: t TValue),
         MapsTo k v m ->
@@ -790,322 +818,319 @@ unfold IndexedTreeConsistency; intros.
     setoid_rewrite Values_fold_perm.
     eexists. eexists.
     rewrite (Partition_fold); eauto.
-   *)
+     *)
 
-  Lemma KeyBasedPartition_fst_singleton :
-    forall {TValue} k v (m: t TValue),
-      MapsTo k v m ->
-      Equal (fst (partition (KeyBasedPartitioningFunction TValue k) m)) (add k v (empty TValue)).
-  Proof.
-    intros.
-    symmetry.
-    unfold Equal; intro key.
+    Lemma KeyBasedPartition_fst_singleton :
+      forall {TValue} k v (m: t TValue),
+        MapsTo k v m ->
+        Equal (fst (partition (KeyBasedPartitioningFunction TValue k) m)) (add k v (empty TValue)).
+    Proof.
+      intros.
+      symmetry.
+      unfold Equal; intro key.
 
-    destruct (E.eq_dec key k) as [ eq_k_proj | neq_k_proj ].
+      destruct (E.eq_dec key k) as [ eq_k_proj | neq_k_proj ].
 
-    rewrite eq_k_proj;
-      rewrite add_eq_o by eauto;
-      symmetry; rewrite <- find_mapsto_iff;
-      rewrite partition_iff_1 with (f := KeyBasedPartitioningFunction TValue k) (m := m);
-      intuition (try rewrite <- KeyBasedPartitioningFunction_eq_true;
-                 eauto using E.eq_refl, KeyBasedPartitioningFunction_Proper).
+      rewrite eq_k_proj;
+        rewrite add_eq_o by eauto;
+        symmetry; rewrite <- find_mapsto_iff;
+        rewrite partition_iff_1 with (f := KeyBasedPartitioningFunction TValue k) (m := m);
+        intuition (try rewrite <- KeyBasedPartitioningFunction_eq_true;
+                   eauto using E.eq_refl, KeyBasedPartitioningFunction_Proper).
 
-    rewrite add_neq_o by eauto.
-    rewrite empty_o.
-    destruct (find key _) eqn:eqfind';
-      [ exfalso | eauto ].
-    rewrite <- find_mapsto_iff in eqfind'.
-    rewrite partition_iff_1 with (f := KeyBasedPartitioningFunction TValue k) (m := m) in eqfind'.
-    destruct eqfind' as (maps_to & kvpf_true).
-    apply neq_k_proj.
-    erewrite KeyBasedPartitioningFunction_eq_true.
-    rewrite KeyBasedPartitioningFunction_refl.
-    eauto.
-    eauto using KeyBasedPartitioningFunction_Proper.
-    reflexivity.
-  Qed.
+      rewrite add_neq_o by eauto.
+      rewrite empty_o.
+      destruct (find key _) eqn:eqfind';
+        [ exfalso | eauto ].
+      rewrite <- find_mapsto_iff in eqfind'.
+      rewrite partition_iff_1 with (f := KeyBasedPartitioningFunction TValue k) (m := m) in eqfind'.
+      destruct eqfind' as (maps_to & kvpf_true).
+      apply neq_k_proj.
+      erewrite KeyBasedPartitioningFunction_eq_true.
+      rewrite KeyBasedPartitioningFunction_refl.
+      eauto.
+      eauto using KeyBasedPartitioningFunction_Proper.
+      reflexivity.
+    Qed.
 
-  Lemma MapsTo_KeyBasedPartition_fst :
-    forall {TValue} k k' v (m: t TValue),
-      MapsTo k' v (fst (partition (KeyBasedPartitioningFunction TValue k) m)) ->
-      E.eq k k'.
-  Proof.
-    intros * maps_to.
-    rewrite partition_iff_1
-    with (f := KeyBasedPartitioningFunction TValue k) (m := m)
-      in maps_to; eauto using KeyBasedPartitioningFunction_Proper.
-    destruct maps_to as (_ & kbpf_true).
-    rewrite <- KeyBasedPartitioningFunction_eq_true in kbpf_true.
-    trivial.
-  Qed.
+    Lemma MapsTo_KeyBasedPartition_fst :
+      forall {TValue} k k' v (m: t TValue),
+        MapsTo k' v (fst (partition (KeyBasedPartitioningFunction TValue k) m)) ->
+        E.eq k k'.
+    Proof.
+      intros * maps_to.
+      rewrite partition_iff_1
+      with (f := KeyBasedPartitioningFunction TValue k) (m := m)
+        in maps_to; eauto using KeyBasedPartitioningFunction_Proper.
+      destruct maps_to as (_ & kbpf_true).
+      rewrite <- KeyBasedPartitioningFunction_eq_true in kbpf_true.
+      trivial.
+    Qed.
 
-  Lemma In_KeyBasedPartition_fst :
-    forall {TValue} k k' (m: t TValue),
-      In k' (fst (partition (KeyBasedPartitioningFunction TValue k) m)) ->
-      E.eq k k'.
-  Proof.
-    intros * in_singleton.
-    apply In_MapsTo in in_singleton.
-    destruct in_singleton as [ val (maps_to & _) ].
-    eapply MapsTo_KeyBasedPartition_fst; eauto.
-  Qed.
+    Lemma In_KeyBasedPartition_fst :
+      forall {TValue} k k' (m: t TValue),
+        In k' (fst (partition (KeyBasedPartitioningFunction TValue k) m)) ->
+        E.eq k k'.
+    Proof.
+      intros * in_singleton.
+      apply In_MapsTo in in_singleton.
+      destruct in_singleton as [ val (maps_to & _) ].
+      eapply MapsTo_KeyBasedPartition_fst; eauto.
+    Qed.
 
-  Lemma MapsTo_KeyBasedPartition_snd :
-    forall {TValue} k k' v (m: t TValue),
-      MapsTo k' v (snd (partition (KeyBasedPartitioningFunction TValue k) m)) ->
-      ~ E.eq k k'.
-  Proof.
-    intros * maps_to.
-    rewrite partition_iff_2
-    with (f := KeyBasedPartitioningFunction TValue k) (m := m)
-      in maps_to; eauto using KeyBasedPartitioningFunction_Proper.
-    destruct maps_to as (_ & kbpf_false).
-    rewrite <- KeyBasedPartitioningFunction_eq_false in kbpf_false.
-    trivial.
-  Qed.
-
-  Lemma In_KeyBasedPartition_snd :
-    forall {TValue} k k' (m: t TValue),
-      In k' (snd (partition (KeyBasedPartitioningFunction TValue k) m)) ->
-      ~ E.eq k k'.
-  Proof.
-    intros * in_falses.
-    apply In_MapsTo in in_falses.
-    destruct in_falses as [ val ( maps_to' & _ ) ].
-    eapply MapsTo_KeyBasedPartition_snd; eauto.
-  Qed.
-
-  Lemma MapsTo_partition_fst:
-    forall TValue f k v (m: t TValue),
-      Proper (E.eq ==> eq ==> eq) f ->
-      MapsTo k v (fst (partition f m)) ->
-      MapsTo k v m.
-  Proof.
-    intros * ? maps_to.
-    rewrite partition_iff_1 with (f := f) (m := m) in maps_to;
-      intuition.
-  Qed.
-
-  Lemma MapsTo_partition_snd:
-    forall TValue f k v (m: t TValue),
-      Proper (E.eq ==> eq ==> eq) f ->
-      MapsTo k v (snd (partition f m)) ->
-      MapsTo k v m.
-  Proof.
-    intros * ? maps_to.
-    rewrite partition_iff_2 with (f := f) (m := m) in maps_to;
-      intuition.
-  Qed.
-
-  Lemma partition_after_KeyBasedPartition_and_add :
-    forall {TValue} k v' (m: t TValue),
-      Partition (add k v' m)
-                (add k v' (fst (partition (KeyBasedPartitioningFunction TValue k) m)))
-                (snd (partition (KeyBasedPartitioningFunction TValue k) m)).
-  Proof.
-    unfold Partition.
-    split.
-
-    {
-      unfold Disjoint.
-      intros key (in_modified & in_unmodified).
-      rewrite add_in_iff in in_modified.
-
-      assert (E.eq k key)
-        by (
-            destruct in_modified;
-            [ assumption | eapply In_KeyBasedPartition_fst; eauto ]
-          ); clear in_modified.
-
-      apply In_KeyBasedPartition_snd in in_unmodified.
-
-      intuition.
-    }
-
-    split; intros * maps_to'.
-    rewrite add_mapsto_iff in maps_to'.
-    destruct maps_to' as [ (keq & veq) | (kneq & maps_to') ]; subst.
-
-    left;
-      apply add_1; eauto.
-    right;
+    Lemma MapsTo_KeyBasedPartition_snd :
+      forall {TValue} k k' v (m: t TValue),
+        MapsTo k' v (snd (partition (KeyBasedPartitioningFunction TValue k) m)) ->
+        ~ E.eq k k'.
+    Proof.
+      intros * maps_to.
       rewrite partition_iff_2
       with (f := KeyBasedPartitioningFunction TValue k) (m := m)
-      by (eauto using KeyBasedPartitioningFunction_Proper);
-      rewrite <- KeyBasedPartitioningFunction_eq_false;
+        in maps_to; eauto using KeyBasedPartitioningFunction_Proper.
+      destruct maps_to as (_ & kbpf_false).
+      rewrite <- KeyBasedPartitioningFunction_eq_false in kbpf_false.
+      trivial.
+    Qed.
+
+    Lemma In_KeyBasedPartition_snd :
+      forall {TValue} k k' (m: t TValue),
+        In k' (snd (partition (KeyBasedPartitioningFunction TValue k) m)) ->
+        ~ E.eq k k'.
+    Proof.
+      intros * in_falses.
+      apply In_MapsTo in in_falses.
+      destruct in_falses as [ val ( maps_to' & _ ) ].
+      eapply MapsTo_KeyBasedPartition_snd; eauto.
+    Qed.
+
+    Lemma MapsTo_partition_fst:
+      forall TValue f k v (m: t TValue),
+        Proper (E.eq ==> eq ==> eq) f ->
+        MapsTo k v (fst (partition f m)) ->
+        MapsTo k v m.
+    Proof.
+      intros * ? maps_to.
+      rewrite partition_iff_1 with (f := f) (m := m) in maps_to;
+        intuition.
+    Qed.
+
+    Lemma MapsTo_partition_snd:
+      forall TValue f k v (m: t TValue),
+        Proper (E.eq ==> eq ==> eq) f ->
+        MapsTo k v (snd (partition f m)) ->
+        MapsTo k v m.
+    Proof.
+      intros * ? maps_to.
+      rewrite partition_iff_2 with (f := f) (m := m) in maps_to;
+        intuition.
+    Qed.
+
+    Lemma partition_after_KeyBasedPartition_and_add :
+      forall {TValue} k v' (m: t TValue),
+        Partition (add k v' m)
+                  (add k v' (fst (partition (KeyBasedPartitioningFunction TValue k) m)))
+                  (snd (partition (KeyBasedPartitioningFunction TValue k) m)).
+    Proof.
+      unfold Partition.
+      split.
+
+      {
+        unfold Disjoint.
+        intros key (in_modified & in_unmodified).
+        rewrite add_in_iff in in_modified.
+
+        assert (E.eq k key)
+          by (
+              destruct in_modified;
+              [ assumption | eapply In_KeyBasedPartition_fst; eauto ]
+            ); clear in_modified.
+
+        apply In_KeyBasedPartition_snd in in_unmodified.
+
+        intuition.
+      }
+
+      split; intros * maps_to'.
+      rewrite add_mapsto_iff in maps_to'.
+      destruct maps_to' as [ (keq & veq) | (kneq & maps_to') ]; subst.
+
+      left;
+        apply add_1; eauto.
+      right;
+        rewrite partition_iff_2
+        with (f := KeyBasedPartitioningFunction TValue k) (m := m)
+        by (eauto using KeyBasedPartitioningFunction_Proper);
+        rewrite <- KeyBasedPartitioningFunction_eq_false;
+        intuition.
+
+      destruct maps_to' as [ maps_to' | maps_to' ].
+
+      rewrite add_mapsto_iff in maps_to';
+        destruct maps_to' as [ (keq & veq) | (kneq & maps_to') ];
+        [ subst; apply add_1; assumption | ].
+
+      exfalso.
+      apply MapsTo_KeyBasedPartition_fst in maps_to'.
       intuition.
 
-    destruct maps_to' as [ maps_to' | maps_to' ].
+      pose proof maps_to'.
+      apply MapsTo_KeyBasedPartition_snd in maps_to'.
+      apply add_2;
+        [ assumption | eapply MapsTo_partition_snd; eauto using KeyBasedPartitioningFunction_Proper ].
+    Qed.
 
-    rewrite add_mapsto_iff in maps_to';
-      destruct maps_to' as [ (keq & veq) | (kneq & maps_to') ];
-      [ subst; apply add_1; assumption | ].
+    Lemma partition_Partition_simple :
+      forall TValue f,
+        Proper (E.eq ==> eq ==> eq) f ->
+        forall (m: t TValue),
+          Partition m
+                    (fst (partition f m))
+                    (snd (partition f m)).
+    Proof.
+      intros.
+      eapply partition_Partition; eauto.
+    Qed.
 
-    exfalso.
-    apply MapsTo_KeyBasedPartition_fst in maps_to'.
-    intuition.
+    Lemma fold_Equal_simpl :
+      forall {TValue TAcc} {eqA: TAcc -> TAcc -> Prop} {m1 m2: t TValue} {f} {init: TAcc},
+        Equal m1 m2 ->
+        Equivalence eqA ->
+        Proper (E.eq ==> eq ==> eqA ==> eqA) f ->
+        transpose_neqkey eqA f ->
+        eqA (fold f m1 init) (fold f m2 init).
+    Proof.
+      intros.
+      apply fold_Equal; assumption.
+    Qed.
 
-    pose proof maps_to'.
-    apply MapsTo_KeyBasedPartition_snd in maps_to'.
-    apply add_2;
-      [ assumption | eapply MapsTo_partition_snd; eauto using KeyBasedPartitioningFunction_Proper ].
-  Qed.
+    Lemma fold_empty :
+      forall {TValue TAcc} f (default: TAcc),
+        fold f (empty TValue) default = default.
+    Proof.
+      intros;
+      apply fold_Empty;
+      eauto using empty_1.
+    Qed.
 
-  Lemma partition_Partition_simple :
-    forall TValue f,
-      Proper (E.eq ==> eq ==> eq) f ->
-      forall (m: t TValue),
-        Partition m
-                  (fst (partition f m))
-                  (snd (partition f m)).
-  Proof.
-    intros.
-    eapply partition_Partition; eauto.
-  Qed.
+    Lemma add_Equal_simple :
+      forall {TValue} {m1 m2: t TValue},
+        Equal m1 m2 ->
+        forall k v,
+          Equal (add k v m1) (add k v m2).
+    Proof.
+      intros.
+      apply add_m; eauto.
+    Qed.
 
-  Lemma fold_Equal_simpl :
-    forall {TValue TAcc} {eqA: TAcc -> TAcc -> Prop} {m1 m2: t TValue} {f} {init: TAcc},
-      Equal m1 m2 ->
-      Equivalence eqA ->
-      Proper (E.eq ==> eq ==> eqA ==> eqA) f ->
-      transpose_neqkey eqA f ->
-      eqA (fold f m1 init) (fold f m2 init).
-  Proof.
-    intros.
-    apply fold_Equal; assumption.
-  Qed.
+    Lemma multiple_adds :
+      forall {TValue} k v1 v2 (m: t TValue),
+        Equal (add k v2 (add k v1 m))
+              (add k v2 m).
+    Proof.
+      intros.
+      unfold Equal.
+      intros k'.
+      destruct (E.eq_dec k k').
 
-  Lemma fold_empty :
-    forall {TValue TAcc} f (default: TAcc),
-      fold f (empty TValue) default = default.
-  Proof.
-    intros;
-    apply fold_Empty;
-    eauto using empty_1.
-  Qed.
+      rewrite !add_eq_o; eauto.
+      rewrite !add_neq_o; eauto.
+    Qed.
 
-  Lemma add_Equal_simple :
-    forall {TValue} {m1 m2: t TValue},
-      Equal m1 m2 ->
-      forall k v,
-        Equal (add k v m1) (add k v m2).
-  Proof.
-    intros.
-    apply add_m; eauto.
-  Qed.
+    Lemma Values_fold_Proper :
+      forall {A},
+        Proper (E.eq ==> eq ==> Permutation (A:=A) ==> Permutation (A:=A))
+               (fun (_ : key) (val : A) (acc : list A) => val :: acc).
+    Proof.
+      unfold Proper, respectful; intros.
+      subst; eauto.
+    Qed.
 
-  Lemma multiple_adds :
-    forall {TValue} k v1 v2 (m: t TValue),
-      Equal (add k v2 (add k v1 m))
-            (add k v2 m).
-  Proof.
-    intros.
-    unfold Equal.
-    intros k'.
-    destruct (E.eq_dec k k').
+    Lemma Values_fold_transpose_neqkey :
+      forall {A},
+        transpose_neqkey (Permutation (A:=A))
+                         (fun (_ : key) (val : A) (acc : list A) => val :: acc).
+    Proof.
+      unfold transpose_neqkey; intros; constructor.
+    Qed.
 
-    rewrite !add_eq_o; eauto.
-    rewrite !add_neq_o; eauto.
-  Qed.
+    Lemma empty_In :
+      forall {TValue} k,
+        ~ In k (empty TValue).
+    Proof.
+      intros; rewrite empty_in_iff; tauto.
+    Qed.
 
-  Lemma Values_fold_Proper :
-    forall {A},
-      Proper (E.eq ==> eq ==> Permutation (A:=A) ==> Permutation (A:=A))
-             (fun (_ : key) (val : A) (acc : list A) => val :: acc).
-  Proof.
-    unfold Proper, respectful; intros.
-    subst; eauto.
-  Qed.
+    Lemma IndexedBag_BagInsertEnumerate :
+      BagInsertEnumerate IndexedBag_benumerate IndexedBag_binsert.
+    Proof.
+      unfold BagInsertEnumerate, IndexedBag_benumerate.
+      intros; simpl in *.
 
-  Lemma Values_fold_transpose_neqkey :
-    forall {A},
-      transpose_neqkey (Permutation (A:=A))
-                       (fun (_ : key) (val : A) (acc : list A) => val :: acc).
-  Proof.
-    unfold transpose_neqkey; intros; constructor.
-  Qed.
+      pose proof bfind_star.
+      unfold BagFindStar in H.
 
-  Lemma empty_In :
-    forall {TValue} k,
-      ~ In k (empty TValue).
-  Proof.
-    intros; rewrite empty_in_iff; tauto.
-  Qed.
+      match goal with
+        | [ |- context[FindWithDefault ?a ?b ?c] ] =>
+          destruct (FindWithDefault_dec a b c)
+            as [ [ result (maps_to & _eq) ] | (find_none & _eq) ];
+            rewrite _eq; clear _eq
+      end.
 
-  Lemma IndexedBag_BagInsertEnumerate :
-    forall {TBag TItem TBagSearchTerm: Type}
-           {bags_bag: Bag TBag TItem TBagSearchTerm}
-           (projection: TItem -> TKey),
-      BagInsertEnumerate IndexedBag_benumerate (IndexedBag_binsert projection).
-  Proof.
-    unfold BagInsertEnumerate, IndexedBag_benumerate.
-    intros; simpl in *.
+      (* Existing key *)
 
-    pose proof bfind_star.
-    unfold BagFindStar in H.
+      pose proof (partition_after_KeyBasedPartition_and_add
+                    (TValue := TBag)
+                    (projection inserted)
+                    (binsert result inserted)
+                    (ifmap container)) as part_add.
 
-    match goal with
-      | [ |- context[FindWithDefault ?a ?b ?c] ] =>
-        destruct (FindWithDefault_dec a b c)
-          as [ [ result (maps_to & _eq) ] | (find_none & _eq) ];
-          rewrite _eq; clear _eq
-    end.
+      pose proof (partition_Partition_simple
+                    (TBag)
+                    (KeyBasedPartitioningFunction TBag (projection inserted))
+                    (KeyBasedPartitioningFunction_Proper _ _)
+                    (ifmap container)) as part.
 
-    (* Existing key *)
+      rewrite !Values_fold_perm
+        by (eauto using Permutation_Equivalence, Values_fold_Proper, Values_fold_transpose_neqkey).
 
-    pose proof (partition_after_KeyBasedPartition_and_add
-                  (TValue := TBag)
-                  (projection inserted)
-                  (binsert result inserted)
-                  (ifmap container)) as part_add.
+      rewrite Partition_fold at 1
+        by (eauto using part_add, Permutation_Equivalence, Values_fold_Proper, Values_fold_transpose_neqkey).
+      symmetry.
 
-    pose proof (partition_Partition_simple
-                  (TBag)
-                  (KeyBasedPartitioningFunction TBag (projection inserted))
-                  (KeyBasedPartitioningFunction_Proper _ _)
-                  (ifmap container)) as part.
+      rewrite Partition_fold at 1
+        by (eauto using part    , Permutation_Equivalence, Values_fold_Proper, Values_fold_transpose_neqkey).
+      symmetry.
 
-    rewrite !Values_fold_perm
-      by (eauto using Permutation_Equivalence, Values_fold_Proper, Values_fold_transpose_neqkey).
+      pose proof (KeyBasedPartition_fst_singleton (TValue := TBag) _ _ _ maps_to) as singleton.
+      pose proof (add_Equal_simple singleton (projection inserted) (binsert result inserted)) as singleton'.
 
-    rewrite Partition_fold at 1
-      by (eauto using part_add, Permutation_Equivalence, Values_fold_Proper, Values_fold_transpose_neqkey).
-    symmetry.
+      rewrite (fold_Equal_simpl (eqA := @Permutation TBag) singleton')
+        by (eauto using Permutation_Equivalence, Values_fold_Proper, Values_fold_transpose_neqkey).
+      rewrite (fold_Equal_simpl (eqA := @Permutation TBag) singleton)
+        by (eauto using Permutation_Equivalence, Values_fold_Proper, Values_fold_transpose_neqkey).
+      rewrite (fold_Equal_simpl (multiple_adds _ _ _ _))
+        by (eauto using Permutation_Equivalence, Values_fold_Proper, Values_fold_transpose_neqkey).
+      rewrite !fold_add
+        by (eauto using Permutation_Equivalence, Values_fold_Proper, Values_fold_transpose_neqkey, empty_In).
 
-    rewrite Partition_fold at 1
-      by (eauto using part    , Permutation_Equivalence, Values_fold_Proper, Values_fold_transpose_neqkey).
-    symmetry.
+      rewrite fold_empty.
 
-    pose proof (KeyBasedPartition_fst_singleton (TValue := TBag) _ _ _ maps_to) as singleton.
-    pose proof (add_Equal_simple singleton (projection inserted) (binsert result inserted)) as singleton'.
+      simpl.
+      rewrite binsert_enumerate.
+      rewrite <- app_comm_cons.
 
-    rewrite (fold_Equal_simpl (eqA := @Permutation TBag) singleton')
-      by (eauto using Permutation_Equivalence, Values_fold_Proper, Values_fold_transpose_neqkey).
-    rewrite (fold_Equal_simpl (eqA := @Permutation TBag) singleton)
-      by (eauto using Permutation_Equivalence, Values_fold_Proper, Values_fold_transpose_neqkey).
-    rewrite (fold_Equal_simpl (multiple_adds _ _ _ _))
-      by (eauto using Permutation_Equivalence, Values_fold_Proper, Values_fold_transpose_neqkey).
-    rewrite !fold_add
-      by (eauto using Permutation_Equivalence, Values_fold_Proper, Values_fold_transpose_neqkey, empty_In).
+      eauto.
 
-    rewrite fold_empty.
+      (* New key *)
 
-    simpl.
-    rewrite binsert_enumerate.
-    rewrite <- app_comm_cons.
+      rewrite <- not_find_in_iff in find_none.
+      rewrite values_add_not_in by assumption.
+      simpl.
 
-    eauto.
-
-    (* New key *)
-
-    rewrite <- not_find_in_iff in find_none.
-    rewrite values_add_not_in by assumption.
-    simpl.
-
-    rewrite binsert_enumerate.
-    rewrite benumerate_empty_eq_nil.
-    simpl; reflexivity.
-  Qed.
+      rewrite binsert_enumerate.
+      rewrite benumerate_empty_eq_nil.
+      simpl; reflexivity.
+    Qed.
 
     Lemma fold_map :
       forall {A B C} seq f g init,
@@ -1127,269 +1152,326 @@ unfold IndexedTreeConsistency; intros.
       reflexivity.
     Qed.
 
-  Lemma IndexedBag_BagCountCorrect :
-    forall {TBag TItem TBagSearchTerm: Type}
-           {bags_bag: Bag TBag TItem TBagSearchTerm}
-           (projection: TItem -> TKey),
-      BagCountCorrect (IndexedBag_bcount projection) (IndexedBag_bfind projection) .
-  Proof.
-    unfold IndexedBag_bcount, IndexedBag_bfind, BagCountCorrect;
-    simpl; intros; destruct search_term as [ [ key | ] search_term ].
-
-    + destruct (find _ _); eauto using bcount_correct.
-    + rewrite length_flatten.
-      rewrite (fold_over_Values _ _ (fun acc bag => acc + bcount bag search_term)) by eauto.
-      rewrite <- fold_left_rev_right.
-      setoid_rewrite Plus.plus_comm at 1.
-      replace (fun (y : TBag) (x : nat) => bcount y search_term + x)
-      with (compose plus (fun bag => bcount bag search_term)) by reflexivity.
-      rewrite !foldright_compose.
-
-      symmetry; setoid_rewrite <- rev_involutive at 1.
-      rewrite fold_left_rev_right, map_rev, rev_involutive.
-
-      rewrite fold_sym, <- !fold_map.
-      setoid_rewrite bcount_correct.
-      reflexivity.
-
-      apply plus_cacheable.
-  Qed.
-
-  Lemma IndexedBag_BagEnumerateEmpty :
-    forall {TBag TItem TBagSearchTerm: Type}
-           {bags_bag: Bag TBag TItem TBagSearchTerm}
-           (projection: TItem -> TKey),
-      BagEnumerateEmpty IndexedBag_benumerate (IndexedBag_bempty projection).
-  Proof.
-    intros;
-    unfold BagEnumerateEmpty, IndexedBag_benumerate, flatten; simpl;
-    rewrite Values_empty; tauto.
-  Qed.
-
-  Lemma IndexedBag_BagFindStar :
-    forall {TBag TItem TBagSearchTerm: Type}
-           {bags_bag: Bag TBag TItem TBagSearchTerm}
-           (projection: TItem -> TKey),
-      BagFindStar (IndexedBag_bfind projection) IndexedBag_benumerate IndexedBag_bstar.
-  Proof.
-    unfold BagFindStar, IndexedBag_benumerate; simpl.
-
-    intros; induction (Values (ifmap container)); simpl; trivial.
-    rewrite (@bfind_star _ _ _ bags_bag).
-    f_equal; trivial.
-  Qed.
-
-  Lemma IndexedBag_BagFindCorrect :
-    forall {TBag TItem TBagSearchTerm: Type}
-           {bags_bag: Bag TBag TItem TBagSearchTerm}
-           (projection: TItem -> TKey),
-      BagFindCorrect (IndexedBag_bfind projection)
-                     (IndexedBag_bfind_matcher projection) IndexedBag_benumerate.
-  Proof.
-    intros.
-    destruct search_term as (option_key, search_term).
-    destruct option_key as [ key | ].
-
-    (* Key provided *)
-
-    unfold IndexedBag_benumerate, IndexedBag_bfind_matcher.
-    pose (iconsistency container).
-    unfold IndexedTreeConsistency in i.
-
-    rewrite filter_and'.
-
-    rewrite flatten_filter.
-
-    Lemma consist :
-      forall
-        {TBag TItem TSearchTerm bags_bag projection}
-        (container: @IndexedBag TBag TItem TSearchTerm bags_bag projection),
-      forall k,
-        eq
-          (flatten
-             (List.map (List.filter (KeyFilter k projection))
-                       (List.map benumerate (Values (ifmap container)))))
-          match find k (ifmap container) with
-            | Some bag => benumerate bag
-            | None => nil
-          end.
+    Lemma fold_plus_sym :
+      forall (seq: list nat) (default: nat),
+        List.fold_right plus default seq =
+        List.fold_left plus seq default.
     Proof.
-      intros.
-
-      pose (iconsistency container); unfold IndexedTreeConsistency in i.
-      unfold Values.
-      destruct (find k (ifmap container)) as [ bag | ] eqn:eqfind.
-
-      rewrite <- find_mapsto_iff in eqfind.
-      (* assert (exists k', MapsTo k' bag (ifmap container)) as eqfind' by (exists k; trivial).*)
-
-      pose proof eqfind as maps_to.
-
-      rewrite elements_mapsto_iff in eqfind.
-      apply InA_split in eqfind.
-
-      destruct eqfind as [ l1 [ y [ l2 (y_k_bag & decomp) ] ] ].
-      rewrite decomp.
-
-      rewrite (map_map snd benumerate).
-      rewrite ! map_app; simpl.
-
-      pose proof (elements_3w (ifmap container)) as no_dup.
-      rewrite decomp in no_dup; apply NoDupA_swap in no_dup; eauto using equiv_eq_key.
-
-      inversion no_dup as [ | ? ? y_not_in no_dup' ]; subst.
-      rewrite InA_app_iff in y_not_in by eauto using equiv_eq_key.
-
-      unfold eq_key_elt in y_k_bag; simpl in y_k_bag.
-      destruct y_k_bag as (y_k & y_bag).
-
-      assert (forall k' bag', InA (@eq_key_elt _) (k', bag') (l1 ++ l2) ->
-                              forall item,
-                                List.In item (benumerate bag') ->
-                                ~ E.eq (projection item) k).
-      {
-        intros k' bag' in_app item in_bag'_items eq_k.
-
-        rewrite InA_app_iff in in_app; eauto using equiv_eq_key_elt.
-        pose proof in_app as in_app'.
-
-        apply (InA_front_tail_InA _ _ y) in in_app.
-        rewrite <- decomp, <- elements_mapsto_iff in in_app.
-
-        pose proof (i _ _ in_app _ in_bag'_items) as eq_k'.
-        symmetry in eq_k.
-        pose proof (E.eq_trans eq_k eq_k').
-
-        assert (eq_key y (k', bag')) as y_eq by (unfold eq_key; simpl; eauto).
-
-        destruct in_app' as [ in_seq | in_seq ];
-          (apply (InA_eqke_eqk (k2 := fst y) (snd y)) in in_seq; eauto);
-          rewrite <- surjective_pairing in in_seq; intuition.
-      }
-
-      Lemma In_InA :
-        forall (A : Type) (l : list A) (eqA : relation A) (x : A),
-          Equivalence eqA -> List.In x l -> InA eqA x l.
-      Proof.
-        induction l; intros; simpl in *.
-        exfalso; eauto using in_nil.
-        destruct H0.
-        apply InA_cons_hd; subst; reflexivity.
-        apply InA_cons_tl, IHl; trivial.
-      Qed.
-
-      rewrite ! map_filter_all_false;
-        [ | intros subseq in_map item in_subseq;
-            rewrite in_map_iff in in_map;
-            destruct in_map as [ (k', bag') (benum_eq & in_seq) ];
-            rewrite KeyFilter_false;
-
-            simpl in benum_eq;
-            subst subseq;
-            apply (H k' bag');
-            eauto;
-
-            apply In_InA; eauto using equiv_eq_key_elt;
-            rewrite in_app_iff;
-            eauto
-              .. ].
-
-      rewrite
-        flatten_app,
-      flatten_head,
-      !flatten_nils,
-      app_nil_l, app_nil_r,
-      <- y_bag,
-      filter_all_true; trivial.
-
-      intros;
-        rewrite KeyFilter_true;
-        apply (iconsistency container _ bag); eauto.
-
-      Lemma nil_in_false :
-        forall {A} seq,
-          seq = nil <-> ~ exists (x: A), List.In x seq.
-      Proof.
-        split; intro H.
-        intros [ x in_seq ]; subst; eauto using in_nil.
-        destruct seq as [ | a ]; trivial.
-        exfalso; apply H; exists a; simpl; intuition.
-      Qed.
-
-      rewrite nil_in_false.
-      intros [item item_in].
-
-      rewrite in_flatten_iff in item_in.
-      do 2 setoid_rewrite in_map_iff in item_in.
-
-      destruct item_in as
-          [ subseq
-              (in_subseq
-                 & [ subseq_prefilter
-                       ( pre_post_filter
-                           & [ bag
-                                 (eq_bag_pre_filter
-                                    & bag_in) ] ) ] ) ].
-
-      subst subseq.
-      rewrite filter_In in in_subseq.
-      destruct in_subseq as (in_subseq_prefilter & key_filter).
-
-      rewrite KeyFilter_true in key_filter.
-      rewrite <- MapsTo_snd in bag_in.
-      destruct bag_in as [k' maps_to].
-
-      subst.
-      rewrite <- key_filter in eqfind.
-      rewrite <- (iconsistency container k' bag maps_to _ in_subseq_prefilter) in maps_to.
-      rewrite find_mapsto_iff in maps_to.
-
-      congruence.
+      intros; rewrite <- fold_left_rev_right.
+      revert default; induction seq; simpl; eauto; intros.
+      rewrite fold_right_app; simpl; rewrite <- IHseq.
+      clear IHseq; revert a default; induction seq;
+      simpl; intros; auto with arith.
+      rewrite <- IHseq; omega.
     Qed.
 
-    simpl.
-    rewrite consist.
-    destruct (find key (ifmap container)) as [ bag | ].
 
-    apply bfind_correct.
-    eauto.
+    Lemma IndexedBag_BagCountCorrect :
+      BagCountCorrect IndexedBag_bcount IndexedBag_bfind .
+    Proof.
+      unfold IndexedBag_bcount, IndexedBag_bfind, BagCountCorrect;
+      simpl; intros; destruct search_term as [ [ key | ] search_term ].
 
-    (* No key provided *)
+      + destruct (find _ _); eauto using bcount_correct.
+      + rewrite length_flatten.
+        rewrite (fold_over_Values _ _ (fun acc bag => acc + bcount bag search_term)) by eauto.
+        rewrite <- fold_left_rev_right.
+        setoid_rewrite Plus.plus_comm at 1.
+        replace (fun (y : TBag) (x : nat) => bcount y search_term + x)
+        with (compose plus (fun bag => bcount bag search_term)) by reflexivity.
+        rewrite !foldright_compose.
 
-    simpl. unfold IndexedBag_benumerate, IndexedBag_bfind_matcher.
-    rewrite flatten_filter.
+        symmetry; setoid_rewrite <- rev_involutive at 1.
+        rewrite fold_left_rev_right, map_rev, rev_involutive.
 
-    induction (Values (ifmap container)); simpl.
+        rewrite fold_plus_sym, <- !fold_map.
+        setoid_rewrite bcount_correct.
+        f_equal;
+          repeat (apply functional_extensionality; intros);
+          auto with arith.
+    Qed.
 
-    eauto.
+    Lemma IndexedBag_BagEnumerateEmpty :
+      BagEnumerateEmpty IndexedBag_benumerate IndexedBag_bempty.
+    Proof.
+      intros;
+      unfold BagEnumerateEmpty, IndexedBag_benumerate, flatten; simpl;
+      rewrite Values_empty; tauto.
+    Qed.
 
-    apply Permutation_app.
-    apply (bfind_correct _).
+    Lemma IndexedBag_BagFindStar :
+      BagFindStar IndexedBag_bfind IndexedBag_benumerate IndexedBag_bstar.
+    Proof.
+      unfold BagFindStar, IndexedBag_benumerate; simpl.
 
-    rewrite IHl; reflexivity.
-  Qed.
+      intros; induction (Values (ifmap container)); simpl; trivial.
+      rewrite bfind_star.
+      f_equal; trivial.
+    Qed.
+
+    Lemma IndexedBag_BagFindCorrect :
+      BagFindCorrect IndexedBag_bfind IndexedBag_bfind_matcher IndexedBag_benumerate.
+    Proof.
+      intros.
+      destruct search_term as (option_key, search_term).
+      destruct option_key as [ key | ].
+
+      (* Key provided *)
+
+      unfold IndexedBag_benumerate, IndexedBag_bfind_matcher.
+      pose (iconsistency container).
+      unfold IndexedTreeConsistency in i.
+
+      rewrite filter_and'.
+
+      rewrite flatten_filter.
+
+      Lemma consist :
+        forall
+          (container: IndexedBag),
+        forall k,
+          eq
+            (flatten
+               (List.map (List.filter (KeyFilter k))
+                         (List.map benumerate (Values (ifmap container)))))
+            match find k (ifmap container) with
+              | Some bag => benumerate bag
+              | None => nil
+            end.
+      Proof.
+        intros.
+
+        pose (iconsistency container); unfold IndexedTreeConsistency in i.
+        unfold Values.
+        destruct (find k (ifmap container)) as [ bag | ] eqn:eqfind.
+
+        rewrite <- find_mapsto_iff in eqfind.
+        (* assert (exists k', MapsTo k' bag (ifmap container)) as eqfind' by (exists k; trivial).*)
+
+        pose proof eqfind as maps_to.
+
+        rewrite elements_mapsto_iff in eqfind.
+        apply InA_split in eqfind.
+
+        destruct eqfind as [ l1 [ y [ l2 (y_k_bag & decomp) ] ] ].
+        rewrite decomp.
+
+        rewrite (map_map snd benumerate).
+        rewrite ! map_app; simpl.
+
+        pose proof (elements_3w (ifmap container)) as no_dup.
+        rewrite decomp in no_dup; apply NoDupA_swap in no_dup; eauto using equiv_eq_key.
+
+        inversion no_dup as [ | ? ? y_not_in no_dup' ]; subst.
+        rewrite InA_app_iff in y_not_in by eauto using equiv_eq_key.
+
+        unfold eq_key_elt in y_k_bag; simpl in y_k_bag.
+        destruct y_k_bag as (y_k & y_bag).
+
+        assert (forall k' bag', InA (@eq_key_elt _) (k', bag') (l1 ++ l2) ->
+                                forall item,
+                                  List.In item (benumerate bag') ->
+                                  ~ E.eq (projection item) k).
+        {
+          intros k' bag' in_app item in_bag'_items eq_k.
+
+          rewrite InA_app_iff in in_app; eauto using equiv_eq_key_elt.
+          pose proof in_app as in_app'.
+
+          apply (InA_front_tail_InA _ _ y) in in_app.
+          rewrite <- decomp, <- elements_mapsto_iff in in_app.
+
+          pose proof (i _ _ in_app _ in_bag'_items) as eq_k'.
+          symmetry in eq_k.
+          pose proof (E.eq_trans eq_k eq_k').
+
+          assert (eq_key y (k', bag')) as y_eq by (unfold eq_key; simpl; eauto).
+
+          destruct in_app' as [ in_seq | in_seq ];
+            (apply (InA_eqke_eqk (k2 := fst y) (snd y)) in in_seq; eauto);
+            rewrite <- surjective_pairing in in_seq; intuition.
+        }
+
+        Lemma In_InA :
+          forall (A : Type) (l : list A) (eqA : relation A) (x : A),
+            Equivalence eqA -> List.In x l -> InA eqA x l.
+        Proof.
+          induction l; intros; simpl in *.
+          exfalso; eauto using in_nil.
+          destruct H0.
+          apply InA_cons_hd; subst; reflexivity.
+          apply InA_cons_tl, IHl; trivial.
+        Qed.
+
+        rewrite ! map_filter_all_false;
+          [ | intros subseq in_map item in_subseq;
+              rewrite in_map_iff in in_map;
+              destruct in_map as [ (k', bag') (benum_eq & in_seq) ];
+              rewrite KeyFilter_false;
+
+              simpl in benum_eq;
+              subst subseq;
+              apply (H k' bag');
+              eauto;
+
+              apply In_InA; eauto using equiv_eq_key_elt;
+              rewrite in_app_iff;
+              eauto
+                .. ].
+
+        rewrite
+          flatten_app,
+        flatten_head,
+        !flatten_nils,
+        app_nil_l, app_nil_r,
+        <- y_bag,
+        filter_all_true; trivial.
+
+        intros;
+          rewrite KeyFilter_true;
+          apply (iconsistency container _ bag); eauto.
+
+        Lemma nil_in_false :
+          forall {A} seq,
+            seq = nil <-> ~ exists (x: A), List.In x seq.
+        Proof.
+          split; intro H.
+          intros [ x in_seq ]; subst; eauto using in_nil.
+          destruct seq as [ | a ]; trivial.
+          exfalso; apply H; exists a; simpl; intuition.
+        Qed.
+
+        rewrite nil_in_false.
+        intros [item item_in].
+
+        rewrite in_flatten_iff in item_in.
+        do 2 setoid_rewrite in_map_iff in item_in.
+
+        destruct item_in as
+            [ subseq
+                (in_subseq
+                   & [ subseq_prefilter
+                         ( pre_post_filter
+                             & [ bag
+                                   (eq_bag_pre_filter
+                                      & bag_in) ] ) ] ) ].
+
+        subst subseq.
+        rewrite filter_In in in_subseq.
+        destruct in_subseq as (in_subseq_prefilter & key_filter).
+
+        rewrite KeyFilter_true in key_filter.
+        rewrite <- MapsTo_snd in bag_in.
+        destruct bag_in as [k' maps_to].
+
+        subst.
+        rewrite <- key_filter in eqfind.
+        rewrite <- (iconsistency container k' bag maps_to _ in_subseq_prefilter) in maps_to.
+        rewrite find_mapsto_iff in maps_to.
+
+        congruence.
+      Qed.
+
+      simpl.
+      rewrite consist.
+      destruct (find key (ifmap container)) as [ bag | ].
+
+      apply bfind_correct.
+      eauto.
+
+      (* No key provided *)
+
+      simpl. unfold IndexedBag_benumerate, IndexedBag_bfind_matcher.
+      rewrite flatten_filter.
+
+      induction (Values (ifmap container)); simpl.
+
+      eauto.
+
+      apply Permutation_app.
+      apply (bfind_correct _).
+
+      rewrite IHl; reflexivity.
+    Qed.
+
+    (* Lemma IndexedBag_BagDeleteCorrect :
+      BagDeleteCorrect IndexedBag_bfind IndexedBag_bfind_matcher
+        IndexedBag_benumerate IndexedBag_bdelete.
+    Proof.
+      unfold BagDeleteCorrect, IndexedBag_bfind, IndexedBag_bfind_matcher,
+      IndexedBag_benumerate, IndexedBag_bdelete, IndexedBag_bdelete'.
+      simpl; intros; case_eq search_term; intros;  case_eq o; simpl; intros; subst.
+      pose proof (bdelete_correct ).
+      case_eq (find t1 (ifmap container)); intros.
+
+      unfold BagDeleteCorrect in H.
+      Check (H (ifmap
+IndexedBag_bcount, IndexedBag_bfind, BagCountCorrect;
+      simpl; intros; destruct search_term as [ [ key | ] search_term ].
+
+      + destruct (find _ _); eauto using bcount_correct.
+      + rewrite length_flatten.
+        rewrite (fold_over_Values _ _ (fun acc bag => acc + bcount bag search_term)) by eauto.
+        rewrite <- fold_left_rev_right.
+        setoid_rewrite Plus.plus_comm at 1.
+        replace (fun (y : TBag) (x : nat) => bcount y search_term + x)
+        with (compose plus (fun bag => bcount bag search_term)) by reflexivity.
+        rewrite !foldright_compose.
+
+        symmetry; setoid_rewrite <- rev_involutive at 1.
+        rewrite fold_left_rev_right, map_rev, rev_involutive.
+
+        rewrite fold_plus_sym, <- !fold_map.
+        setoid_rewrite bcount_correct.
+        f_equal;
+          repeat (apply functional_extensionality; intros);
+          auto with arith.
+    Qed. *)
+
+
+  End TreeBagDefinitions.
 
   Instance IndexedBagAsBag
-           (TBag TItem TBagSearchTerm: Type)
-           (bags_bag: Bag TBag TItem TBagSearchTerm) (projection: TItem -> TKey)
-  : Bag
-      (@IndexedBag TBag TItem TBagSearchTerm bags_bag projection)
-      TItem
-      ((option TKey) * TBagSearchTerm) :=
-    {|
-      bempty        := IndexedBag_bempty projection;
-      bstar         := IndexedBag_bstar;
-      bfind_matcher := IndexedBag_bfind_matcher projection;
+           (TBag TItem TBagSearchTerm TBagUpdateTerm: Type)
+           (projection: TItem -> TKey)
+           (bags_bag : @KeyPreservingUpdateBag
+                         TBag TItem TBagSearchTerm
+                         TBagUpdateTerm projection)
+  : @KeyPreservingUpdateBag _ TItem _ TBagUpdateTerm projection :=
+    {| KeyPreserving_bag :=
+         {| bempty            := IndexedBag_bempty projection bags_bag;
+            bstar             := IndexedBag_bstar projection bags_bag;
+            bid               := bid;
+            bfind_matcher     := IndexedBag_bfind_matcher projection bags_bag;
+            bupdate_transform := bupdate_transform;
 
-      benumerate := IndexedBag_benumerate;
-      bfind      := IndexedBag_bfind projection;
-      binsert    := IndexedBag_binsert projection;
-      bcount     := IndexedBag_bcount projection;
+            benumerate := IndexedBag_benumerate projection bags_bag;
+            bfind      := IndexedBag_bfind projection bags_bag;
+            binsert    := IndexedBag_binsert projection bags_bag;
+            bcount     := IndexedBag_bcount projection bags_bag;
+            bdelete    := IndexedBag_bdelete projection bags_bag;
+            bupdate    := IndexedBag_bupdate projection bags_bag;
 
-      binsert_enumerate := IndexedBag_BagInsertEnumerate projection;
-      benumerate_empty  := IndexedBag_BagEnumerateEmpty projection;
-      bfind_star        := IndexedBag_BagFindStar projection;
-      bfind_correct     := IndexedBag_BagFindCorrect projection;
-      bcount_correct    := IndexedBag_BagCountCorrect projection
-    |}.
+            binsert_enumerate := IndexedBag_BagInsertEnumerate projection bags_bag;
+            benumerate_empty  := IndexedBag_BagEnumerateEmpty projection bags_bag;
+            bfind_star        := IndexedBag_BagFindStar projection bags_bag;
+            bfind_correct     := IndexedBag_BagFindCorrect projection bags_bag;
+            bcount_correct    := IndexedBag_BagCountCorrect projection bags_bag
+            (* bdelete_correct   := IndexedBag_BagDeleteCorrect projection bags_bag; 
+            bupdate_correct   := IndexedBag_BagUpdateCorrect projection bags_bag *)
+
+         |} |}.
+  Proof.
+    simpl.
+    unfold bupdate_transform.
+    destruct bags_bag; destruct KeyPreserving_bag0; simpl in *; intros.
+    eapply KeyPreserving_Proof0 with (searchTerm := snd searchTerm); eauto.
+    unfold IndexedBag_bfind_matcher in H0; simpl in *.
+    destruct searchTerm; destruct o; simpl in *; eauto.
+    destruct (bfind_matcher t0 item); eauto.
+    destruct (KeyFilter projection t1 item); simpl in *; discriminate.
+  Abort. 
+  (* Still Missing the two correctness proofs. *)
+
+    
 End TreeBag.
